<?xml version="1.0"?>
<rdf:RDF xmlns="http://www.ontologylibrary.mil/OperationalEnvironment/Mid/OEOrganizationOntology#"
     xml:base="http://www.ontologylibrary.mil/OperationalEnvironment/Mid/OEOrganizationOntology"
	xmlns:dc="http://purl.org/dc/elements/1.1/"
  	xmlns:cco="http://www.ontologyrepository.com/CommonCoreOntologies/"
	xmlns:obo="http://purl.obolibrary.org/obo/"
	xmlns:owl="http://www.w3.org/2002/07/owl#"
	xmlns:rdf="http://www.w3.org/1999/02/22-rdf-syntax-ns#"
	xmlns:xml="http://www.w3.org/XML/1998/namespace"
	xmlns:xsd="http://www.w3.org/2001/XMLSchema#"
	xmlns:foaf="http://xmlns.com/foaf/0.1/"
	xmlns:rdfs="http://www.w3.org/2000/01/rdf-schema#"
	xmlns:event="http://www.ontologylibrary.mil/OperationalEnvironment/Mid/OEEventOntology#">

    <owl:Ontology rdf:about="http://www.ontologylibrary.mil/OperationalEnvironment/Mid/OEOrganizationOntology">
	<owl:imports rdf:resource="http://www.ontologyrepository.com/CommonCoreOntologies/Mid/AgentOntology"/>
	<owl:imports rdf:resource="http://www.ontologyrepository.com/CommonCoreOntologies/Upper/ExtendedRelationOntology"/>
	<owl:versionInfo rdf:datatype="http://www.w3.org/2001/XMLSchema#string">DISTRIBUTION A: Approved for public release; distribution is unlimited.  For more information contact United States Army TRADOC G-27 at usarmy.jble.tradoc.list.tboc-operations@mail.mil (or Kaye Darone, Data Science Branch Chief, DSMS, Kaye.t.darone.civ@mail.mil, (757) 878-9547)</owl:versionInfo>
	<owl:versionInfo rdf:datatype="http://www.w3.org/2001/XMLSchema#string">Version 3.1</owl:versionInfo>
	<owl:versionInfo rdf:datatype="http://www.w3.org/2001/XMLSchema#string">Sep 21, 2017</owl:versionInfo>
    </owl:Ontology>
<!--  -->
<!--  -->
<!-- ################################################################# -->
<!-- # -->
<!-- #    Classes -->
<!-- # -->
<!-- ################################################################# -->
<!--  -->
<!--  -->
<!-- http://www.ontologylibrary.mil/OperationalEnvironment/Mid/OEOrganizationOntology#Agriculture -->

<rdf:Description rdf:about="http://www.ontologylibrary.mil/OperationalEnvironment/Mid/OEOrganizationOntology#Agriculture">
	<rdf:type rdf:resource="http://www.w3.org/2002/07/owl#Class"/>
	<rdfs:subClassOf rdf:resource="http://www.ontologyrepository.com/CommonCoreOntologies/Organization"/>
	<rdfs:comment>Definition: Agriculture: individuals and groups involved in the practices of crop cultivation
including government agencies whose primary concern is agricultural issues</rdfs:comment>
	<rdfs:label>Agriculture</rdfs:label>
</rdf:Description>
<!--  -->
<!-- http://www.ontologylibrary.mil/OperationalEnvironment/Mid/OEOrganizationOntology#Business -->

<rdf:Description rdf:about="http://www.ontologylibrary.mil/OperationalEnvironment/Mid/OEOrganizationOntology#Business">
	<rdf:type rdf:resource="http://www.w3.org/2002/07/owl#Class"/>
	<rdfs:subClassOf rdf:resource="http://www.ontologyrepository.com/CommonCoreOntologies/Organization"/>
	<rdfs:comment>Definition: Business: businessmen, companies, and enterprises, not including MNCs</rdfs:comment>
	<rdfs:label>Business</rdfs:label>
</rdf:Description>
<!--  -->
<!-- http://www.ontologylibrary.mil/OperationalEnvironment/Mid/OEOrganizationOntology#Civilian -->

<rdf:Description rdf:about="http://www.ontologylibrary.mil/OperationalEnvironment/Mid/OEOrganizationOntology#Civilian">
	<rdf:type rdf:resource="http://www.w3.org/2002/07/owl#Class"/>
	<rdfs:subClassOf rdf:resource="http://www.ontologyrepository.com/CommonCoreOntologies/Organization"/>
	<rdfs:comment>Definition: Civilian individuals or groups sometimes used as catch-all for individuals or
groups for whom no other role category is appropriate</rdfs:comment>
	<rdfs:label>Civilian</rdfs:label>
</rdf:Description>
<!--  -->
<!-- http://www.ontologylibrary.mil/OperationalEnvironment/Mid/OEOrganizationOntology#Criminal -->

<rdf:Description rdf:about="http://www.ontologylibrary.mil/OperationalEnvironment/Mid/OEOrganizationOntology#Criminal">
	<rdf:type rdf:resource="http://www.w3.org/2002/07/owl#Class"/>
	<rdfs:subClassOf rdf:resource="http://www.ontologyrepository.com/CommonCoreOntologies/Organization"/>
	<rdfs:comment>Definition: Criminal: corresponding to individuals involved in or allegedly involved in the
deliberate breaking of state or international laws primarily for profit</rdfs:comment>
	<rdfs:label>Criminal</rdfs:label>
</rdf:Description>
<!--  -->
<!-- http://www.ontologylibrary.mil/OperationalEnvironment/Mid/OEOrganizationOntology#Development -->

<rdf:Description rdf:about="http://www.ontologylibrary.mil/OperationalEnvironment/Mid/OEOrganizationOntology#Development">
	<rdf:type rdf:resource="http://www.w3.org/2002/07/owl#Class"/>
	<rdfs:subClassOf rdf:resource="http://www.ontologyrepository.com/CommonCoreOntologies/Organization"/>
	<rdfs:comment>Definition: Development: individuals or groups concerned primarily with development
issues of varying types including infrastructure creation, democratization et al.</rdfs:comment>
	<rdfs:label>Development</rdfs:label>
</rdf:Description>
<!--  -->
<!-- http://www.ontologylibrary.mil/OperationalEnvironment/Mid/OEOrganizationOntology#Education -->

<rdf:Description rdf:about="http://www.ontologylibrary.mil/OperationalEnvironment/Mid/OEOrganizationOntology#Education">
	<rdf:type rdf:resource="http://www.w3.org/2002/07/owl#Class"/>
	<rdfs:subClassOf rdf:resource="http://www.ontologyrepository.com/CommonCoreOntologies/Organization"/>
	<rdfs:comment>Definition: Education: educators, schools, students, or organizations dealing with education</rdfs:comment>
	<rdfs:label>Education</rdfs:label>
</rdf:Description>
<!--  -->
<!-- http://www.ontologylibrary.mil/OperationalEnvironment/Mid/OEOrganizationOntology#Elites -->

<rdf:Description rdf:about="http://www.ontologylibrary.mil/OperationalEnvironment/Mid/OEOrganizationOntology#Elites">
	<rdf:type rdf:resource="http://www.w3.org/2002/07/owl#Class"/>
	<rdfs:subClassOf rdf:resource="http://www.ontologyrepository.com/CommonCoreOntologies/Organization"/>
	<rdfs:comment>Definition: Elites: former government officials, celebrities, spokespersons for organizations
without further role categorization (George Soros, former Secretary of Defense, Bono)</rdfs:comment>
	<rdfs:label>Elites</rdfs:label>
</rdf:Description>
<!--  -->
<!-- http://www.ontologylibrary.mil/OperationalEnvironment/Mid/OEOrganizationOntology#Environmental -->

<rdf:Description rdf:about="http://www.ontologylibrary.mil/OperationalEnvironment/Mid/OEOrganizationOntology#Environmental">
	<rdf:type rdf:resource="http://www.w3.org/2002/07/owl#Class"/>
	<rdfs:subClassOf rdf:resource="http://www.ontologyrepository.com/CommonCoreOntologies/Organization"/>
	<rdfs:comment>Definition: Environmental: entities for whom environmental and ecological issues are
their primary focus, includes wildlife preservation, climate change, etc.</rdfs:comment>
	<rdfs:label>Environmental</rdfs:label>
</rdf:Description>
<!--  -->
<!-- http://www.ontologylibrary.mil/OperationalEnvironment/Mid/OEOrganizationOntology#Executive -->

<rdf:Description rdf:about="http://www.ontologylibrary.mil/OperationalEnvironment/Mid/OEOrganizationOntology#Executive">
	<rdf:type rdf:resource="http://www.w3.org/2002/07/owl#Class"/>
	<rdfs:subClassOf rdf:resource="http://www.ontologyrepository.com/CommonCoreOntologies/Government"/>
	<rdfs:comment>Definition: Executive: Elected and non-elected officials and supporting organizations. The executive is the organ exercising authority in and holding responsibility for the governance of a state. The executive executes and enforces law.</rdfs:comment>
	<rdfs:label>Executive</rdfs:label>
</rdf:Description>
<!--  -->
<!-- http://www.ontologylibrary.mil/OperationalEnvironment/Mid/OEOrganizationOntology#Health -->

<rdf:Description rdf:about="http://www.ontologylibrary.mil/OperationalEnvironment/Mid/OEOrganizationOntology#Health">
	<rdf:type rdf:resource="http://www.w3.org/2002/07/owl#Class"/>
	<rdfs:subClassOf rdf:resource="http://www.ontologyrepository.com/CommonCoreOntologies/Organization"/>
	<rdfs:comment>Definition: Health: individuals, groups and organizations dealing with health and social
welfare practices (doctors, Doctors Without Borders)</rdfs:comment>
	<rdfs:label>Health</rdfs:label>
</rdf:Description>
<!--  -->
<!-- http://www.ontologylibrary.mil/OperationalEnvironment/Mid/OEOrganizationOntology#HumanRights -->

<rdf:Description rdf:about="http://www.ontologylibrary.mil/OperationalEnvironment/Mid/OEOrganizationOntology#HumanRights">
	<rdf:type rdf:resource="http://www.w3.org/2002/07/owl#Class"/>
	<rdfs:subClassOf rdf:resource="http://www.ontologyrepository.com/CommonCoreOntologies/Organization"/>
	<rdfs:comment>Definition: Human Rights: actors for whom their primary area of operation or expertise
is with documenting and/or correcting human rights concerns</rdfs:comment>
	<rdfs:label>Human Rights</rdfs:label>
</rdf:Description>
<!--  -->
<!-- http://www.ontologylibrary.mil/OperationalEnvironment/Mid/OEOrganizationOntology#Insurgent -->

<rdf:Description rdf:about="http://www.ontologylibrary.mil/OperationalEnvironment/Mid/OEOrganizationOntology#Insurgent">
	<rdf:type rdf:resource="http://www.w3.org/2002/07/owl#Class"/>
	<rdfs:subClassOf rdf:resource="http://www.ontologylibrary.mil/OperationalEnvironment/Mid/OEOrganizationOntology#Rebels"/>
	<rdfs:comment>Definition: Insurgents (rebels): all rebels who attempt to overthrow their national government</rdfs:comment>
	<rdfs:label>Insurgent</rdfs:label>
</rdf:Description>
<!--  -->
<!-- http://www.ontologylibrary.mil/OperationalEnvironment/Mid/OEOrganizationOntology#Judiciary -->

<rdf:Description rdf:about="http://www.ontologylibrary.mil/OperationalEnvironment/Mid/OEOrganizationOntology#Judiciary">
	<rdf:type rdf:resource="http://www.w3.org/2002/07/owl#Class"/>
	<rdfs:subClassOf rdf:resource="http://www.ontologyrepository.com/CommonCoreOntologies/Government"/>
	<rdfs:comment>Definition: Judiciary: judges, courts</rdfs:comment>
	<rdfs:label>Judiciary</rdfs:label>
</rdf:Description>
<!--  -->
<!-- http://www.ontologylibrary.mil/OperationalEnvironment/Mid/OEOrganizationOntology#Labor -->

<rdf:Description rdf:about="http://www.ontologylibrary.mil/OperationalEnvironment/Mid/OEOrganizationOntology#Labor">
	<rdf:type rdf:resource="http://www.w3.org/2002/07/owl#Class"/>
	<rdfs:subClassOf rdf:resource="http://www.ontologyrepository.com/CommonCoreOntologies/Organization"/>
	<rdfs:comment>Definition: Labor: specifcally individuals in or elements of organized labor, organizations
concerned with labor issues</rdfs:comment>
	<rdfs:label>Labor</rdfs:label>
</rdf:Description>
<!--  -->
<!-- http://www.ontologylibrary.mil/OperationalEnvironment/Mid/OEOrganizationOntology#Legislature -->

<rdf:Description rdf:about="http://www.ontologylibrary.mil/OperationalEnvironment/Mid/OEOrganizationOntology#Legislature">
	<rdf:type rdf:resource="http://www.w3.org/2002/07/owl#Class"/>
	<rdfs:subClassOf rdf:resource="http://www.ontologyrepository.com/CommonCoreOntologies/Government"/>
	<rdfs:comment>Definition: Legislature: parliaments, assemblies, lawmakers, references to specific
legislative entities or sub-entities such as committees</rdfs:comment>
	<rdfs:label>Legislature</rdfs:label>
</rdf:Description>
<!--  -->
<!-- http://www.ontologylibrary.mil/OperationalEnvironment/Mid/OEOrganizationOntology#Media -->

<rdf:Description rdf:about="http://www.ontologylibrary.mil/OperationalEnvironment/Mid/OEOrganizationOntology#Media">
	<rdf:type rdf:resource="http://www.w3.org/2002/07/owl#Class"/>
	<rdfs:subClassOf rdf:resource="http://www.ontologyrepository.com/CommonCoreOntologies/Organization"/>
	<rdfs:comment>Definition: Media: journalists, newspapers, television stations also includes providers of
internet services and other forms of mass information dissemination</rdfs:comment>
	<rdfs:label>Media</rdfs:label>
</rdf:Description>
<!--  -->
<!-- http://www.ontologylibrary.mil/OperationalEnvironment/Mid/OEOrganizationOntology#Police -->

<rdf:Description rdf:about="http://www.ontologylibrary.mil/OperationalEnvironment/Mid/OEOrganizationOntology#Police">
	<rdf:type rdf:resource="http://www.w3.org/2002/07/owl#Class"/>
	<rdfs:subClassOf rdf:resource="http://www.ontologyrepository.com/CommonCoreOntologies/Organization"/>
	<rdfs:comment>Definition: Police forces, officers, criminal investigative units, protective agencies</rdfs:comment>
	<rdfs:label>Police</rdfs:label>
</rdf:Description>
<!--  -->
<!-- http://www.ontologylibrary.mil/OperationalEnvironment/Mid/OEOrganizationOntology#PoliticalOpposition -->

<rdf:Description rdf:about="http://www.ontologylibrary.mil/OperationalEnvironment/Mid/OEOrganizationOntology#PoliticalOpposition">
	<rdf:type rdf:resource="http://www.w3.org/2002/07/owl#Class"/>
	<rdfs:subClassOf rdf:resource="http://www.ontologyrepository.com/CommonCoreOntologies/Organization"/>
	<rdfs:comment>Definition: Political opposition: opposition parties, individuals, anti-government activists</rdfs:comment>
	<rdfs:label>Political Opposition</rdfs:label>
</rdf:Description>
<!--  -->
<!-- http://www.ontologylibrary.mil/OperationalEnvironment/Mid/OEOrganizationOntology#Rebels -->

<rdf:Description rdf:about="http://www.ontologylibrary.mil/OperationalEnvironment/Mid/OEOrganizationOntology#Rebels">
	<rdf:type rdf:resource="http://www.w3.org/2002/07/owl#Class"/>
	<rdfs:subClassOf rdf:resource="http://www.ontologyrepository.com/CommonCoreOntologies/Organization"/>
	<rdfs:comment>Definition: Rebels: armed and violent opposition groups, individuals</rdfs:comment>
	<rdfs:label>Rebels</rdfs:label>
</rdf:Description>
<!--  -->
<!-- http://www.ontologylibrary.mil/OperationalEnvironment/Mid/OEOrganizationOntology#Refugees -->

<rdf:Description rdf:about="http://www.ontologylibrary.mil/OperationalEnvironment/Mid/OEOrganizationOntology#Refugees">
	<rdf:type rdf:resource="http://www.w3.org/2002/07/owl#Class"/>
	<rdfs:subClassOf rdf:resource="http://www.ontologyrepository.com/CommonCoreOntologies/Organization"/>
	<rdfs:comment>Definition: Refugees: also refers to agencies or MNCs dealing with population migration
and relocation issues</rdfs:comment>
	<rdfs:label>Refugees</rdfs:label>
</rdf:Description>
<!--  -->
<!-- http://www.ontologylibrary.mil/OperationalEnvironment/Mid/OEOrganizationOntology#Religious -->

<rdf:Description rdf:about="http://www.ontologylibrary.mil/OperationalEnvironment/Mid/OEOrganizationOntology#Religious">
	<rdf:type rdf:resource="http://www.w3.org/2002/07/owl#Class"/>
	<rdfs:subClassOf rdf:resource="http://www.ontologyrepository.com/CommonCoreOntologies/Organization"/>
	<rdfs:subClassOf rdf:nodeID="genid1"/>
</rdf:Description>

<rdf:Description rdf:nodeID="genid1">
	<rdf:type rdf:resource="http://www.w3.org/2002/07/owl#Restriction"/>
	<owl:onProperty rdf:resource="http://www.ontologyrepository.com/CommonCoreOntologies/aggregate_has_quality"/>
	<owl:someValuesFrom rdf:resource="http://www.ontologyrepository.com/CommonCoreOntologies/Ethnicity"/>
</rdf:Description>

<rdf:Description rdf:about="http://www.ontologylibrary.mil/OperationalEnvironment/Mid/OEOrganizationOntology#Religious">
	<rdfs:comment>Definition: Organizations or groups specifically tied to a Religious philosopy.</rdfs:comment>
	<rdfs:label>Religious</rdfs:label>
</rdf:Description>
<!--  -->
<!-- http://www.ontologylibrary.mil/OperationalEnvironment/Mid/OEOrganizationOntology#Separatist -->

<rdf:Description rdf:about="http://www.ontologylibrary.mil/OperationalEnvironment/Mid/OEOrganizationOntology#Separatist">
	<rdf:type rdf:resource="http://www.w3.org/2002/07/owl#Class"/>
	<rdfs:subClassOf rdf:resource="http://www.ontologylibrary.mil/OperationalEnvironment/Mid/OEOrganizationOntology#Rebels"/>
	<rdfs:comment>Definition: Separatist rebels: all rebels who try to emancipate their region from its country</rdfs:comment>
	<rdfs:label>Separatist</rdfs:label>
</rdf:Description>
<!--  -->
<!-- http://www.ontologylibrary.mil/OperationalEnvironment/Mid/OEOrganizationOntology#Spy -->

<rdf:Description rdf:about="http://www.ontologylibrary.mil/OperationalEnvironment/Mid/OEOrganizationOntology#Spy">
	<rdf:type rdf:resource="http://www.w3.org/2002/07/owl#Class"/>
	<rdfs:subClassOf rdf:resource="http://www.ontologyrepository.com/CommonCoreOntologies/Organization"/>
	<rdfs:comment>Definition: State intelligence services and members including covert operations groups
as well as intelligence collection and analyses</rdfs:comment>
	<rdfs:label>Spy</rdfs:label>
</rdf:Description>
<!--  -->
<!-- http://www.ontologylibrary.mil/OperationalEnvironment/Mid/OEOrganizationOntology#UnalignedArmedForces -->

<rdf:Description rdf:about="http://www.ontologylibrary.mil/OperationalEnvironment/Mid/OEOrganizationOntology#UnalignedArmedForces">
	<rdf:type rdf:resource="http://www.w3.org/2002/07/owl#Class"/>
	<rdfs:subClassOf rdf:resource="http://www.ontologyrepository.com/CommonCoreOntologies/ArmedForce"/>
	<rdfs:comment>Definition: Armed forces aligned neither with nor against their government</rdfs:comment>
	<rdfs:label>Unaligned Armed Force</rdfs:label>
</rdf:Description>
<!--  -->
<!-- Generated by the OWL API (version 4.2.6.20160910-2108) https://github.com/owlcs/owlapi -->

</rdf:RDF>
