<?xml version="1.0"?>


<!DOCTYPE rdf:RDF [
    <!ENTITY owl "http://www.w3.org/2002/07/owl#" >
    <!ENTITY obo "http://purl.obolibrary.org/obo/" >
    <!ENTITY xsd "http://www.w3.org/2001/XMLSchema#" >
    <!ENTITY rdfs "http://www.w3.org/2000/01/rdf-schema#" >
    <!ENTITY rdf "http://www.w3.org/1999/02/22-rdf-syntax-ns#" >
    <!ENTITY ero "http://www.ontologylibrary.mil/CommonCore/Upper/ExtendedRelationOntology#" >
]>


<rdf:RDF xmlns="http://www.ontologylibrary.mil/CommonCore/Mid/QualityOntology#"
     xml:base="http://www.ontologylibrary.mil/CommonCore/Mid/QualityOntology"
     xmlns:obo="http://purl.obolibrary.org/obo/"
     xmlns:rdfs="http://www.w3.org/2000/01/rdf-schema#"
     xmlns:owl="http://www.w3.org/2002/07/owl#"
     xmlns:xsd="http://www.w3.org/2001/XMLSchema#"
     xmlns:rdf="http://www.w3.org/1999/02/22-rdf-syntax-ns#"
     xmlns:ero="http://www.ontologylibrary.mil/CommonCore/Upper/ExtendedRelationOntology#">
    <owl:Ontology rdf:about="http://www.ontologylibrary.mil/CommonCore/Mid/QualityOntology">
        <owl:versionInfo rdf:datatype="&xsd;string">February 17, 2016</owl:versionInfo>
        <owl:versionInfo rdf:datatype="&xsd;string">Version 0.85.2</owl:versionInfo>
		<owl:versionInfo rdf:datatype="&xsd;string">COPYRIGHT Â© 2015 CUBRC, Inc.</owl:versionInfo>
        <owl:imports rdf:resource="http://www.ontologylibrary.mil/CommonCore/Upper/ExtendedRelationOntology"/>
    </owl:Ontology>
    


    <!-- 
    ///////////////////////////////////////////////////////////////////////////////////////
    //
    // Classes
    //
    ///////////////////////////////////////////////////////////////////////////////////////
     -->

    


    <!-- http://www.ontologylibrary.mil/CommonCore/Mid/QualityOntology#AbsorptionQuality -->

    <owl:Class rdf:about="http://www.ontologylibrary.mil/CommonCore/Mid/QualityOntology#AbsorptionQuality">
        <rdfs:label>Absorption Quality</rdfs:label>
        <rdfs:subClassOf rdf:resource="http://www.ontologylibrary.mil/CommonCore/Mid/QualityOntology#FullSpectrumElectromagneticRadiationQuality"/>
        <rdfs:comment>A scalar EM radiation quality which obtains by the capacity of the bearer to retain radiation.</rdfs:comment>
    </owl:Class>
    


    <!-- http://www.ontologylibrary.mil/CommonCore/Mid/QualityOntology#AbsorptionWavelength -->

    <owl:Class rdf:about="http://www.ontologylibrary.mil/CommonCore/Mid/QualityOntology#AbsorptionWavelength">
        <rdfs:label>Absorption Wavelength</rdfs:label>
        <rdfs:subClassOf rdf:resource="http://www.ontologylibrary.mil/CommonCore/Mid/QualityOntology#AbsorptionQuality"/>
        <rdfs:comment>The specific wavelength of radiation that can be retained by a bearer.</rdfs:comment>
    </owl:Class>
    


    <!-- http://www.ontologylibrary.mil/CommonCore/Mid/QualityOntology#Albedo -->

    <owl:Class rdf:about="http://www.ontologylibrary.mil/CommonCore/Mid/QualityOntology#Albedo">
        <rdfs:label>Albedo</rdfs:label>
        <rdfs:subClassOf rdf:resource="http://www.ontologylibrary.mil/CommonCore/Mid/QualityOntology#RadiationReflectiveQuality"/>
        <rdfs:comment>A reflective quality restricted to a particular wavelength.</rdfs:comment>
    </owl:Class>
    


    <!-- http://www.ontologylibrary.mil/CommonCore/Mid/QualityOntology#Amount -->

    <owl:Class rdf:about="http://www.ontologylibrary.mil/CommonCore/Mid/QualityOntology#Amount">
        <rdfs:label rdf:datatype="&xsd;string">Amount</rdfs:label>
        <rdfs:subClassOf rdf:resource="&obo;BFO_0000019"/>
        <rdfs:comment rdf:datatype="&xsd;string">A Quality that inheres in some Entity by virtue of the total, aggregate or sum of a number of discrete items or material the entity contains as parts. (derived from http://en.wiktionary.org/wiki/amount)</rdfs:comment>
    </owl:Class>
    


    <!-- http://www.ontologylibrary.mil/CommonCore/Mid/QualityOntology#Angular -->

    <owl:Class rdf:about="http://www.ontologylibrary.mil/CommonCore/Mid/QualityOntology#Angular">
        <rdfs:label>Angular</rdfs:label>
        <rdfs:subClassOf rdf:resource="http://www.ontologylibrary.mil/CommonCore/Mid/QualityOntology#Shape"/>
        <rdfs:comment>A shape quality inhering in a bearer by virtue of the bearer&apos;s having at least one salient angle on the margin.</rdfs:comment>
    </owl:Class>
    


    <!-- http://www.ontologylibrary.mil/CommonCore/Mid/QualityOntology#ArrowShaped -->

    <owl:Class rdf:about="http://www.ontologylibrary.mil/CommonCore/Mid/QualityOntology#ArrowShaped">
        <rdfs:label>ArrowShaped</rdfs:label>
        <rdfs:subClassOf rdf:resource="http://www.ontologylibrary.mil/CommonCore/Mid/QualityOntology#Shape"/>
        <rdfs:comment>A shape quality inhering in a bearer by virtue of the bearer&apos;s forming two equal obtuse triangles with a short side in common.</rdfs:comment>
    </owl:Class>
    


    <!-- http://www.ontologylibrary.mil/CommonCore/Mid/QualityOntology#Auburn -->

    <owl:Class rdf:about="http://www.ontologylibrary.mil/CommonCore/Mid/QualityOntology#Auburn">
        <rdfs:label rdf:datatype="&xsd;string">Auburn</rdfs:label>
        <owl:equivalentClass rdf:resource="http://www.ontologylibrary.mil/CommonCore/Mid/QualityOntology#RedBrown"/>
        <rdfs:subClassOf rdf:resource="http://www.ontologylibrary.mil/CommonCore/Mid/QualityOntology#ColorHue"/>
        <rdfs:comment rdf:datatype="&xsd;string">Definition: A synonym of RedBrown</rdfs:comment>
    </owl:Class>
    


    <!-- http://www.ontologylibrary.mil/CommonCore/Mid/QualityOntology#Autofluorescence -->

    <owl:Class rdf:about="http://www.ontologylibrary.mil/CommonCore/Mid/QualityOntology#Autofluorescence">
        <rdfs:label>Autofluorescence</rdfs:label>
        <rdfs:subClassOf rdf:resource="http://www.ontologylibrary.mil/CommonCore/Mid/QualityOntology#Fluorescence"/>
        <rdfs:comment>A fluorescence quality inhering in a bearer by virtue of the bearer&apos;s exhibiting fluorescence which is self-induced.</rdfs:comment>
    </owl:Class>
    


    <!-- http://www.ontologylibrary.mil/CommonCore/Mid/QualityOntology#Bent -->

    <owl:Class rdf:about="http://www.ontologylibrary.mil/CommonCore/Mid/QualityOntology#Bent">
        <rdfs:label>Bent</rdfs:label>
        <rdfs:subClassOf rdf:resource="http://www.ontologylibrary.mil/CommonCore/Mid/QualityOntology#Shape"/>
        <rdfs:comment>A shape quality inhering in a bearer by virtue of the bearer&apos;s having one or more angle(s) in its length.</rdfs:comment>
    </owl:Class>
    


    <!-- http://www.ontologylibrary.mil/CommonCore/Mid/QualityOntology#Black -->

    <owl:Class rdf:about="http://www.ontologylibrary.mil/CommonCore/Mid/QualityOntology#Black">
        <rdfs:label>Black</rdfs:label>
        <rdfs:subClassOf rdf:resource="http://www.ontologylibrary.mil/CommonCore/Mid/QualityOntology#ColorHue"/>
        <rdfs:comment>A color that lacks any hues as parts.</rdfs:comment>
    </owl:Class>
    


    <!-- http://www.ontologylibrary.mil/CommonCore/Mid/QualityOntology#Blond -->

    <owl:Class rdf:about="http://www.ontologylibrary.mil/CommonCore/Mid/QualityOntology#Blond">
        <rdfs:label rdf:datatype="&xsd;string">Blond</rdfs:label>
        <rdfs:subClassOf rdf:resource="http://www.ontologylibrary.mil/CommonCore/Mid/QualityOntology#ColorHue"/>
        <rdfs:comment rdf:datatype="&xsd;string">Definition: A Color that ranges from nearly white to a light greyish yellow</rdfs:comment>
    </owl:Class>
    


    <!-- http://www.ontologylibrary.mil/CommonCore/Mid/QualityOntology#Blue -->

    <owl:Class rdf:about="http://www.ontologylibrary.mil/CommonCore/Mid/QualityOntology#Blue">
        <rdfs:label>Blue</rdfs:label>
        <rdfs:subClassOf rdf:resource="http://www.ontologylibrary.mil/CommonCore/Mid/QualityOntology#ColorHue"/>
        <rdfs:comment>A color hue with low wavelength of that portion of the visible spectrum lying between green and indigo, evoked in the human observer by radiant energy with wavelengths of approximately 420 to 490 nanometers.</rdfs:comment>
    </owl:Class>
    


    <!-- http://www.ontologylibrary.mil/CommonCore/Mid/QualityOntology#Blunt -->

    <owl:Class rdf:about="http://www.ontologylibrary.mil/CommonCore/Mid/QualityOntology#Blunt">
        <rdfs:label>Blunt</rdfs:label>
        <rdfs:subClassOf rdf:resource="http://www.ontologylibrary.mil/CommonCore/Mid/QualityOntology#Sharpness"/>
        <rdfs:comment>A shape quality inhering in a bearer by virtue of the bearer&apos;s terminating gradually in a rounded end.</rdfs:comment>
    </owl:Class>
    


    <!-- http://www.ontologylibrary.mil/CommonCore/Mid/QualityOntology#Blurry -->

    <owl:Class rdf:about="http://www.ontologylibrary.mil/CommonCore/Mid/QualityOntology#Blurry">
        <rdfs:label>Blurry</rdfs:label>
        <rdfs:subClassOf rdf:resource="http://www.ontologylibrary.mil/CommonCore/Mid/QualityOntology#Focus"/>
        <rdfs:comment>An optical quality inhering in a bearer by virtue of the bearer&apos;s lacking focus.</rdfs:comment>
    </owl:Class>
    


    <!-- http://www.ontologylibrary.mil/CommonCore/Mid/QualityOntology#Branched -->

    <owl:Class rdf:about="http://www.ontologylibrary.mil/CommonCore/Mid/QualityOntology#Branched">
        <rdfs:label>Branched</rdfs:label>
        <rdfs:subClassOf rdf:resource="http://www.ontologylibrary.mil/CommonCore/Mid/QualityOntology#Branchiness"/>
        <rdfs:comment>A branchiness quality inhering in a bearer by virtue of the bearer&apos;s having branches.</rdfs:comment>
    </owl:Class>
    


    <!-- http://www.ontologylibrary.mil/CommonCore/Mid/QualityOntology#Branchiness -->

    <owl:Class rdf:about="http://www.ontologylibrary.mil/CommonCore/Mid/QualityOntology#Branchiness">
        <rdfs:label>Branchiness</rdfs:label>
        <rdfs:subClassOf rdf:resource="http://www.ontologylibrary.mil/CommonCore/Mid/QualityOntology#Shape"/>
        <rdfs:comment>A shape quality inhering in a bearer by virtue of the degree to which there are subdivisions or offshoots in a bearer entity.</rdfs:comment>
    </owl:Class>
    


    <!-- http://www.ontologylibrary.mil/CommonCore/Mid/QualityOntology#Brown -->

    <owl:Class rdf:about="http://www.ontologylibrary.mil/CommonCore/Mid/QualityOntology#Brown">
        <rdfs:label>Brown</rdfs:label>
        <rdfs:subClassOf rdf:resource="http://www.ontologylibrary.mil/CommonCore/Mid/QualityOntology#ColorHue"/>
        <rdfs:comment>A color consisting of dark orange, red, of very low intensity.</rdfs:comment>
    </owl:Class>
    


    <!-- http://www.ontologylibrary.mil/CommonCore/Mid/QualityOntology#BrownGreen -->

    <owl:Class rdf:about="http://www.ontologylibrary.mil/CommonCore/Mid/QualityOntology#BrownGreen">
        <rdfs:label>Brown Green</rdfs:label>
        <owl:equivalentClass rdf:resource="http://www.ontologylibrary.mil/CommonCore/Mid/QualityOntology#Hazel"/>
        <rdfs:subClassOf rdf:resource="http://www.ontologylibrary.mil/CommonCore/Mid/QualityOntology#Green"/>
        <rdfs:comment>A color consisting of brown and green hues.</rdfs:comment>
    </owl:Class>
    


    <!-- http://www.ontologylibrary.mil/CommonCore/Mid/QualityOntology#Circumference -->

    <owl:Class rdf:about="http://www.ontologylibrary.mil/CommonCore/Mid/QualityOntology#Circumference">
        <rdfs:label>Circumference</rdfs:label>
        <rdfs:subClassOf rdf:resource="http://www.ontologylibrary.mil/CommonCore/Mid/QualityOntology#Perimeter"/>
        <rdfs:comment>An 1D extent quality which is equal to the length of the closed curve of a circle.</rdfs:comment>
    </owl:Class>
    


    <!-- http://www.ontologylibrary.mil/CommonCore/Mid/QualityOntology#Closed -->

    <owl:Class rdf:about="http://www.ontologylibrary.mil/CommonCore/Mid/QualityOntology#Closed">
        <rdfs:label>Closed</rdfs:label>
        <rdfs:subClassOf rdf:resource="http://www.ontologylibrary.mil/CommonCore/Mid/QualityOntology#Closure"/>
        <rdfs:comment>A morphological quality inhering in a bearer by virtue of the bearer&apos;s affording blocked passage or view.</rdfs:comment>
    </owl:Class>
    


    <!-- http://www.ontologylibrary.mil/CommonCore/Mid/QualityOntology#Closure -->

    <owl:Class rdf:about="http://www.ontologylibrary.mil/CommonCore/Mid/QualityOntology#Closure">
        <rdfs:label>Closure</rdfs:label>
        <rdfs:subClassOf rdf:resource="http://www.ontologylibrary.mil/CommonCore/Mid/QualityOntology#MorphologicalQuality"/>
        <rdfs:comment>A morphological quality pertaining to the degree to which an object contains an opening aperture orifice or vent.</rdfs:comment>
    </owl:Class>
    


    <!-- http://www.ontologylibrary.mil/CommonCore/Mid/QualityOntology#ClosureIncomplete -->

    <owl:Class rdf:about="http://www.ontologylibrary.mil/CommonCore/Mid/QualityOntology#ClosureIncomplete">
        <rdfs:label>Closure Incomplete</rdfs:label>
        <rdfs:subClassOf rdf:resource="http://www.ontologylibrary.mil/CommonCore/Mid/QualityOntology#Open"/>
        <rdfs:comment>A morphological quality inhering in a bearer by virtue of the bearer&apos;s affording not completed blocked passage or view.</rdfs:comment>
    </owl:Class>
    


    <!-- http://www.ontologylibrary.mil/CommonCore/Mid/QualityOntology#Coiled -->

    <owl:Class rdf:about="http://www.ontologylibrary.mil/CommonCore/Mid/QualityOntology#Coiled">
        <rdfs:label>Coiled</rdfs:label>
        <rdfs:subClassOf rdf:resource="http://www.ontologylibrary.mil/CommonCore/Mid/QualityOntology#Coiling"/>
        <rdfs:comment>A shape quality inhering in a bearer by virtue of the bearer&apos;s being curled or wound (especially in concentric rings or spirals).</rdfs:comment>
    </owl:Class>
    


    <!-- http://www.ontologylibrary.mil/CommonCore/Mid/QualityOntology#Coiling -->

    <owl:Class rdf:about="http://www.ontologylibrary.mil/CommonCore/Mid/QualityOntology#Coiling">
        <rdfs:label>Coiling</rdfs:label>
        <rdfs:subClassOf rdf:resource="http://www.ontologylibrary.mil/CommonCore/Mid/QualityOntology#Shape"/>
        <rdfs:comment>A shape quality inhering in a bearer by virtue of the bearer&apos;s being wound in a continuous series of loops.</rdfs:comment>
    </owl:Class>
    


    <!-- http://www.ontologylibrary.mil/CommonCore/Mid/QualityOntology#ColorBrightness -->

    <owl:Class rdf:about="http://www.ontologylibrary.mil/CommonCore/Mid/QualityOntology#ColorBrightness">
        <rdfs:label>Color Brightness</rdfs:label>
        <rdfs:subClassOf rdf:resource="http://www.ontologylibrary.mil/CommonCore/Mid/QualityOntology#OpticalQuality"/>
        <rdfs:comment>A scalar optical property that is the intensity, value or amount of perceived light.</rdfs:comment>
    </owl:Class>
    


    <!-- http://www.ontologylibrary.mil/CommonCore/Mid/QualityOntology#ColorHue -->

    <owl:Class rdf:about="http://www.ontologylibrary.mil/CommonCore/Mid/QualityOntology#ColorHue">
        <rdfs:label>Color Hue</rdfs:label>
        <rdfs:subClassOf rdf:resource="http://www.ontologylibrary.mil/CommonCore/Mid/QualityOntology#OpticalQuality"/>
        <rdfs:comment>A composite chromatic quality composed of hue, saturation and intensity parts.</rdfs:comment>
    </owl:Class>
    


    <!-- http://www.ontologylibrary.mil/CommonCore/Mid/QualityOntology#ColorSaturation -->

    <owl:Class rdf:about="http://www.ontologylibrary.mil/CommonCore/Mid/QualityOntology#ColorSaturation">
        <rdfs:label>Color Saturation</rdfs:label>
        <rdfs:subClassOf rdf:resource="http://www.ontologylibrary.mil/CommonCore/Mid/QualityOntology#OpticalQuality"/>
        <rdfs:comment>A scalar chromatic property that is the degree of purity of perceived light.</rdfs:comment>
    </owl:Class>
    


    <!-- http://www.ontologylibrary.mil/CommonCore/Mid/QualityOntology#Colored -->

    <owl:Class rdf:about="http://www.ontologylibrary.mil/CommonCore/Mid/QualityOntology#Colored">
        <rdfs:label>Colored</rdfs:label>
        <rdfs:subClassOf rdf:resource="http://www.ontologylibrary.mil/CommonCore/Mid/QualityOntology#ColorHue"/>
        <rdfs:comment>A color quality inhering in a bearer by virtue of the bearer&apos;s having color.</rdfs:comment>
    </owl:Class>
    


    <!-- http://www.ontologylibrary.mil/CommonCore/Mid/QualityOntology#Concave -->

    <owl:Class rdf:about="http://www.ontologylibrary.mil/CommonCore/Mid/QualityOntology#Concave">
        <rdfs:label>Concave 3D Shape</rdfs:label>
        <rdfs:subClassOf rdf:resource="http://www.ontologylibrary.mil/CommonCore/Mid/QualityOntology#Shape"/>
        <rdfs:comment>A complete three dimensional shape in which there is a line connecting a pair of points on the object that lies outside the object. Or: a shape with cavities. Contrast: concave.</rdfs:comment>
    </owl:Class>
    


    <!-- http://www.ontologylibrary.mil/CommonCore/Mid/QualityOntology#Convex -->

    <owl:Class rdf:about="http://www.ontologylibrary.mil/CommonCore/Mid/QualityOntology#Convex">
        <rdfs:label>Convex 3D Shape</rdfs:label>
        <rdfs:subClassOf rdf:resource="http://www.ontologylibrary.mil/CommonCore/Mid/QualityOntology#Shape"/>
        <rdfs:comment>A complete three dimensional shape in which for every line connecting a pair of points on the object is within the object. Or: a shape lacking cavities. Contrast: concave.</rdfs:comment>
    </owl:Class>
    


    <!-- http://www.ontologylibrary.mil/CommonCore/Mid/QualityOntology#CrescentShaped -->

    <owl:Class rdf:about="http://www.ontologylibrary.mil/CommonCore/Mid/QualityOntology#CrescentShaped">
        <rdfs:label>CrescentShaped</rdfs:label>
        <rdfs:subClassOf rdf:resource="http://www.ontologylibrary.mil/CommonCore/Mid/QualityOntology#TwoDimensionalShape"/>
        <rdfs:comment>A shape quality inhering in a circular disk by virtue of the bearer&apos;s having a segment of another circle removed from its edge so that what remains is a shape enclosed by two circular arcs of different diameters which intersect at two points (usually in such a manner that the enclosed shape does not include the center of the original circle).</rdfs:comment>
    </owl:Class>
    


    <!-- http://www.ontologylibrary.mil/CommonCore/Mid/QualityOntology#CubeShaped -->

    <owl:Class rdf:about="http://www.ontologylibrary.mil/CommonCore/Mid/QualityOntology#CubeShaped">
        <rdfs:subClassOf rdf:resource="http://www.ontologylibrary.mil/CommonCore/Mid/QualityOntology#ThreeDimensionalShape"/>
    </owl:Class>
    


    <!-- http://www.ontologylibrary.mil/CommonCore/Mid/QualityOntology#Curled -->

    <owl:Class rdf:about="http://www.ontologylibrary.mil/CommonCore/Mid/QualityOntology#Curled">
        <rdfs:label>Curled</rdfs:label>
        <rdfs:subClassOf rdf:resource="http://www.ontologylibrary.mil/CommonCore/Mid/QualityOntology#Shape"/>
        <rdfs:comment>A shape quality inhering in a bearer by virtue of the bearer&apos;s having parallel chains in undulate fashion on the border.</rdfs:comment>
    </owl:Class>
    


    <!-- http://www.ontologylibrary.mil/CommonCore/Mid/QualityOntology#Curved -->

    <owl:Class rdf:about="http://www.ontologylibrary.mil/CommonCore/Mid/QualityOntology#Curved">
        <rdfs:label>Curved</rdfs:label>
        <rdfs:subClassOf rdf:resource="http://www.ontologylibrary.mil/CommonCore/Mid/QualityOntology#Shape"/>
        <rdfs:comment>A curvature quality inhering in a bearer by virtue of the bearer&apos;s having or being marked by a curve or smoothly rounded bend.</rdfs:comment>
    </owl:Class>
    


    <!-- http://www.ontologylibrary.mil/CommonCore/Mid/QualityOntology#Cyan -->

    <owl:Class rdf:about="http://www.ontologylibrary.mil/CommonCore/Mid/QualityOntology#Cyan">
        <rdfs:label>Cyan</rdfs:label>
        <rdfs:subClassOf rdf:resource="http://www.ontologylibrary.mil/CommonCore/Mid/QualityOntology#ColorHue"/>
        <rdfs:comment>A color consisting of green and blue hue.</rdfs:comment>
    </owl:Class>
    


    <!-- http://www.ontologylibrary.mil/CommonCore/Mid/QualityOntology#Cylindrical -->

    <owl:Class rdf:about="http://www.ontologylibrary.mil/CommonCore/Mid/QualityOntology#Cylindrical">
        <rdfs:label>Columnar</rdfs:label>
        <rdfs:subClassOf rdf:resource="http://www.ontologylibrary.mil/CommonCore/Mid/QualityOntology#ThreeDimensionalShape"/>
        <rdfs:comment>A shape inhering in a bearer by virtue of the bearer&apos;s being elongated and cylindrical.</rdfs:comment>
    </owl:Class>
    


    <!-- http://www.ontologylibrary.mil/CommonCore/Mid/QualityOntology#DarkBlue -->

    <owl:Class rdf:about="http://www.ontologylibrary.mil/CommonCore/Mid/QualityOntology#DarkBlue">
        <rdfs:label>Dark Blue</rdfs:label>
        <rdfs:subClassOf rdf:resource="http://www.ontologylibrary.mil/CommonCore/Mid/QualityOntology#Blue"/>
        <rdfs:comment>A color consisting of blue hue and low brightness.</rdfs:comment>
    </owl:Class>
    


    <!-- http://www.ontologylibrary.mil/CommonCore/Mid/QualityOntology#DarkBrown -->

    <owl:Class rdf:about="http://www.ontologylibrary.mil/CommonCore/Mid/QualityOntology#DarkBrown">
        <rdfs:label>Dark Brown</rdfs:label>
        <rdfs:subClassOf rdf:resource="http://www.ontologylibrary.mil/CommonCore/Mid/QualityOntology#Brown"/>
        <rdfs:comment>A color consisting of brown hue and low brightness.</rdfs:comment>
    </owl:Class>
    


    <!-- http://www.ontologylibrary.mil/CommonCore/Mid/QualityOntology#DarkCyan -->

    <owl:Class rdf:about="http://www.ontologylibrary.mil/CommonCore/Mid/QualityOntology#DarkCyan">
        <rdfs:label>Dark Cyan</rdfs:label>
        <rdfs:subClassOf rdf:resource="http://www.ontologylibrary.mil/CommonCore/Mid/QualityOntology#Cyan"/>
        <rdfs:comment>A color consisting of cyan hue and low brightness.</rdfs:comment>
    </owl:Class>
    


    <!-- http://www.ontologylibrary.mil/CommonCore/Mid/QualityOntology#DarkGreen -->

    <owl:Class rdf:about="http://www.ontologylibrary.mil/CommonCore/Mid/QualityOntology#DarkGreen">
        <rdfs:label>Dark Green</rdfs:label>
        <rdfs:subClassOf rdf:resource="http://www.ontologylibrary.mil/CommonCore/Mid/QualityOntology#Green"/>
        <rdfs:comment>A color consisting of green hue and low brightness.</rdfs:comment>
    </owl:Class>
    


    <!-- http://www.ontologylibrary.mil/CommonCore/Mid/QualityOntology#DarkGrey -->

    <owl:Class rdf:about="http://www.ontologylibrary.mil/CommonCore/Mid/QualityOntology#DarkGrey">
        <rdfs:label>Dark Grey</rdfs:label>
        <rdfs:subClassOf rdf:resource="http://www.ontologylibrary.mil/CommonCore/Mid/QualityOntology#Grey"/>
        <rdfs:comment>A color consisting of grey color and low brightness.</rdfs:comment>
    </owl:Class>
    


    <!-- http://www.ontologylibrary.mil/CommonCore/Mid/QualityOntology#DarkMagenta -->

    <owl:Class rdf:about="http://www.ontologylibrary.mil/CommonCore/Mid/QualityOntology#DarkMagenta">
        <rdfs:label>Dark Magenta</rdfs:label>
        <rdfs:subClassOf rdf:resource="http://www.ontologylibrary.mil/CommonCore/Mid/QualityOntology#Magenta"/>
        <rdfs:comment>A color consisting of magenta with low brightness.</rdfs:comment>
    </owl:Class>
    


    <!-- http://www.ontologylibrary.mil/CommonCore/Mid/QualityOntology#DarkOrange -->

    <owl:Class rdf:about="http://www.ontologylibrary.mil/CommonCore/Mid/QualityOntology#DarkOrange">
        <rdfs:label>Dark Orange</rdfs:label>
        <rdfs:subClassOf rdf:resource="http://www.ontologylibrary.mil/CommonCore/Mid/QualityOntology#Orange"/>
        <rdfs:comment>A color consisting of orange color and low brightness.</rdfs:comment>
    </owl:Class>
    


    <!-- http://www.ontologylibrary.mil/CommonCore/Mid/QualityOntology#DarkPalePink -->

    <owl:Class rdf:about="http://www.ontologylibrary.mil/CommonCore/Mid/QualityOntology#DarkPalePink">
        <rdfs:label>Dark Pale Pink</rdfs:label>
        <rdfs:subClassOf rdf:resource="http://www.ontologylibrary.mil/CommonCore/Mid/QualityOntology#Pink"/>
        <rdfs:comment>Pink color having medium brightness and low saturation.</rdfs:comment>
    </owl:Class>
    


    <!-- http://www.ontologylibrary.mil/CommonCore/Mid/QualityOntology#DarkPurple -->

    <owl:Class rdf:about="http://www.ontologylibrary.mil/CommonCore/Mid/QualityOntology#DarkPurple">
        <rdfs:label>Dark Purple</rdfs:label>
        <rdfs:subClassOf rdf:resource="http://www.ontologylibrary.mil/CommonCore/Mid/QualityOntology#Purple"/>
        <rdfs:comment>A color consisting of purple color and low brightness.</rdfs:comment>
    </owl:Class>
    


    <!-- http://www.ontologylibrary.mil/CommonCore/Mid/QualityOntology#DarkRed -->

    <owl:Class rdf:about="http://www.ontologylibrary.mil/CommonCore/Mid/QualityOntology#DarkRed">
        <rdfs:label>Dark Red</rdfs:label>
        <rdfs:subClassOf rdf:resource="http://www.ontologylibrary.mil/CommonCore/Mid/QualityOntology#Red"/>
        <rdfs:comment>A color consisting of red hue and low brightness.</rdfs:comment>
    </owl:Class>
    


    <!-- http://www.ontologylibrary.mil/CommonCore/Mid/QualityOntology#DarkRedBrown -->

    <owl:Class rdf:about="http://www.ontologylibrary.mil/CommonCore/Mid/QualityOntology#DarkRedBrown">
        <rdfs:label>Dark Red Brown</rdfs:label>
        <rdfs:subClassOf rdf:resource="http://www.ontologylibrary.mil/CommonCore/Mid/QualityOntology#RedBrown"/>
        <rdfs:comment>A color consisting of red and brown hue and low brightness.</rdfs:comment>
    </owl:Class>
    


    <!-- http://www.ontologylibrary.mil/CommonCore/Mid/QualityOntology#DarkViolet -->

    <owl:Class rdf:about="http://www.ontologylibrary.mil/CommonCore/Mid/QualityOntology#DarkViolet">
        <rdfs:label>Dark Violet</rdfs:label>
        <rdfs:subClassOf rdf:resource="http://www.ontologylibrary.mil/CommonCore/Mid/QualityOntology#Violet"/>
        <rdfs:comment>A color consisting of violet hue and low brightness.</rdfs:comment>
    </owl:Class>
    


    <!-- http://www.ontologylibrary.mil/CommonCore/Mid/QualityOntology#DarkYellow -->

    <owl:Class rdf:about="http://www.ontologylibrary.mil/CommonCore/Mid/QualityOntology#DarkYellow">
        <rdfs:label>Dark Yellow</rdfs:label>
        <rdfs:subClassOf rdf:resource="http://www.ontologylibrary.mil/CommonCore/Mid/QualityOntology#Yellow"/>
        <rdfs:comment>A color consisting of yellow hue and low brightness.</rdfs:comment>
    </owl:Class>
    


    <!-- http://www.ontologylibrary.mil/CommonCore/Mid/QualityOntology#DeepPink -->

    <owl:Class rdf:about="http://www.ontologylibrary.mil/CommonCore/Mid/QualityOntology#DeepPink">
        <rdfs:label>Deep Pink</rdfs:label>
        <rdfs:subClassOf rdf:resource="http://www.ontologylibrary.mil/CommonCore/Mid/QualityOntology#Pink"/>
        <rdfs:comment>Pink color having medium brightness and moderate saturation.</rdfs:comment>
    </owl:Class>
    


    <!-- http://www.ontologylibrary.mil/CommonCore/Mid/QualityOntology#Density -->

    <owl:Class rdf:about="http://www.ontologylibrary.mil/CommonCore/Mid/QualityOntology#Density">
        <rdfs:label>Mass Density</rdfs:label>
        <rdfs:subClassOf rdf:resource="http://www.ontologylibrary.mil/CommonCore/Mid/QualityOntology#PhysicalQuality"/>
        <rdfs:comment>A physical quality which inheres in a bearer by virtue of some influence is exerted by the bearer&apos;s mass per unit size.</rdfs:comment>
    </owl:Class>
    


    <!-- http://www.ontologylibrary.mil/CommonCore/Mid/QualityOntology#Depth -->

    <owl:Class rdf:about="http://www.ontologylibrary.mil/CommonCore/Mid/QualityOntology#Depth">
        <rdfs:label>Depth</rdfs:label>
        <rdfs:subClassOf rdf:resource="http://www.ontologylibrary.mil/CommonCore/Mid/QualityOntology#OneDimensionalExtent"/>
        <rdfs:comment>A 1D extent quality inhering in a bearer by virtue of the bearer&apos;s downward or backward or inward dimenision.</rdfs:comment>
    </owl:Class>
    


    <!-- http://www.ontologylibrary.mil/CommonCore/Mid/QualityOntology#DesaturatedBlue -->

    <owl:Class rdf:about="http://www.ontologylibrary.mil/CommonCore/Mid/QualityOntology#DesaturatedBlue">
        <rdfs:label>Desaturated Blue</rdfs:label>
        <rdfs:subClassOf rdf:resource="http://www.ontologylibrary.mil/CommonCore/Mid/QualityOntology#Blue"/>
        <rdfs:comment>A color consisting of blue hue and low saturation.</rdfs:comment>
    </owl:Class>
    


    <!-- http://www.ontologylibrary.mil/CommonCore/Mid/QualityOntology#DesaturatedBrown -->

    <owl:Class rdf:about="http://www.ontologylibrary.mil/CommonCore/Mid/QualityOntology#DesaturatedBrown">
        <rdfs:label>Desaturated Brown</rdfs:label>
        <rdfs:subClassOf rdf:resource="http://www.ontologylibrary.mil/CommonCore/Mid/QualityOntology#Brown"/>
        <rdfs:comment>A color consisting of brown hue and low saturation.</rdfs:comment>
    </owl:Class>
    


    <!-- http://www.ontologylibrary.mil/CommonCore/Mid/QualityOntology#DesaturatedCyan -->

    <owl:Class rdf:about="http://www.ontologylibrary.mil/CommonCore/Mid/QualityOntology#DesaturatedCyan">
        <rdfs:label>Desaturated Cyan</rdfs:label>
        <rdfs:subClassOf rdf:resource="http://www.ontologylibrary.mil/CommonCore/Mid/QualityOntology#Cyan"/>
        <rdfs:comment>A color consisting of cyan colour and low saturation.</rdfs:comment>
    </owl:Class>
    


    <!-- http://www.ontologylibrary.mil/CommonCore/Mid/QualityOntology#DesaturatedGreen -->

    <owl:Class rdf:about="http://www.ontologylibrary.mil/CommonCore/Mid/QualityOntology#DesaturatedGreen">
        <rdfs:label>Desaturated Green</rdfs:label>
        <rdfs:subClassOf rdf:resource="http://www.ontologylibrary.mil/CommonCore/Mid/QualityOntology#Green"/>
        <rdfs:comment>A color consisting of green hue and low saturation.</rdfs:comment>
    </owl:Class>
    


    <!-- http://www.ontologylibrary.mil/CommonCore/Mid/QualityOntology#DesaturatedMagenta -->

    <owl:Class rdf:about="http://www.ontologylibrary.mil/CommonCore/Mid/QualityOntology#DesaturatedMagenta">
        <rdfs:label>Desaturated Magenta</rdfs:label>
        <rdfs:subClassOf rdf:resource="http://www.ontologylibrary.mil/CommonCore/Mid/QualityOntology#Magenta"/>
        <rdfs:comment>A color consisting of magenta color and low saturation.</rdfs:comment>
    </owl:Class>
    


    <!-- http://www.ontologylibrary.mil/CommonCore/Mid/QualityOntology#DesaturatedOrange -->

    <owl:Class rdf:about="http://www.ontologylibrary.mil/CommonCore/Mid/QualityOntology#DesaturatedOrange">
        <rdfs:label>Desaturated Orange</rdfs:label>
        <rdfs:subClassOf rdf:resource="http://www.ontologylibrary.mil/CommonCore/Mid/QualityOntology#Orange"/>
        <rdfs:comment>A color consisting of orange hue and low saturation.</rdfs:comment>
    </owl:Class>
    


    <!-- http://www.ontologylibrary.mil/CommonCore/Mid/QualityOntology#DesaturatedPurple -->

    <owl:Class rdf:about="http://www.ontologylibrary.mil/CommonCore/Mid/QualityOntology#DesaturatedPurple">
        <rdfs:label>Desaturated Purple</rdfs:label>
        <rdfs:subClassOf rdf:resource="http://www.ontologylibrary.mil/CommonCore/Mid/QualityOntology#Purple"/>
        <rdfs:comment>A color consisting of purple color and low saturation.</rdfs:comment>
    </owl:Class>
    


    <!-- http://www.ontologylibrary.mil/CommonCore/Mid/QualityOntology#DesaturatedRed -->

    <owl:Class rdf:about="http://www.ontologylibrary.mil/CommonCore/Mid/QualityOntology#DesaturatedRed">
        <rdfs:label>Desaturated Red</rdfs:label>
        <rdfs:subClassOf rdf:resource="http://www.ontologylibrary.mil/CommonCore/Mid/QualityOntology#Red"/>
        <rdfs:comment>A color consisting of red hue and low saturation.</rdfs:comment>
    </owl:Class>
    


    <!-- http://www.ontologylibrary.mil/CommonCore/Mid/QualityOntology#DesaturatedViolet -->

    <owl:Class rdf:about="http://www.ontologylibrary.mil/CommonCore/Mid/QualityOntology#DesaturatedViolet">
        <rdfs:label>Desaturated Violet</rdfs:label>
        <rdfs:subClassOf rdf:resource="http://www.ontologylibrary.mil/CommonCore/Mid/QualityOntology#Violet"/>
        <rdfs:comment>A color consisting of violet hue and low saturation.</rdfs:comment>
    </owl:Class>
    


    <!-- http://www.ontologylibrary.mil/CommonCore/Mid/QualityOntology#DesaturatedYellow -->

    <owl:Class rdf:about="http://www.ontologylibrary.mil/CommonCore/Mid/QualityOntology#DesaturatedYellow">
        <rdfs:label>Desaturated Yellow</rdfs:label>
        <rdfs:subClassOf rdf:resource="http://www.ontologylibrary.mil/CommonCore/Mid/QualityOntology#Yellow"/>
        <rdfs:comment>A color consisting of yellow hue and low saturation.</rdfs:comment>
    </owl:Class>
    


    <!-- http://www.ontologylibrary.mil/CommonCore/Mid/QualityOntology#Diameter -->

    <owl:Class rdf:about="http://www.ontologylibrary.mil/CommonCore/Mid/QualityOntology#Diameter">
        <rdfs:label>Diameter</rdfs:label>
        <rdfs:subClassOf rdf:resource="http://www.ontologylibrary.mil/CommonCore/Mid/QualityOntology#Length"/>
        <rdfs:comment>A length quality which is equal to the length of any straight line segment that passes through the center of a circle and whose endpoints are on the circular boundary.</rdfs:comment>
    </owl:Class>
    


    <!-- http://www.ontologylibrary.mil/CommonCore/Mid/QualityOntology#Drooping -->

    <owl:Class rdf:about="http://www.ontologylibrary.mil/CommonCore/Mid/QualityOntology#Drooping">
        <rdfs:label>Drooping</rdfs:label>
        <rdfs:subClassOf rdf:resource="http://www.ontologylibrary.mil/CommonCore/Mid/QualityOntology#Shape"/>
        <rdfs:comment rdf:datatype="&xsd;string">To bend or hang downwards.</rdfs:comment>
    </owl:Class>
    


    <!-- http://www.ontologylibrary.mil/CommonCore/Mid/QualityOntology#Dry -->

    <owl:Class rdf:about="http://www.ontologylibrary.mil/CommonCore/Mid/QualityOntology#Dry">
        <rdfs:label>Dry</rdfs:label>
        <rdfs:subClassOf rdf:resource="http://www.ontologylibrary.mil/CommonCore/Mid/QualityOntology#Wetness"/>
        <rdfs:comment>A wetness quality inhering in a bearer by virtue of the bearer&apos;s not being covered by a liquid.</rdfs:comment>
    </owl:Class>
    


    <!-- http://www.ontologylibrary.mil/CommonCore/Mid/QualityOntology#ElectromagneticRadiationQuality -->

    <owl:Class rdf:about="http://www.ontologylibrary.mil/CommonCore/Mid/QualityOntology#ElectromagneticRadiationQuality">
        <rdfs:label>Electromagnetic (Em) Radiation Quality</rdfs:label>
        <rdfs:subClassOf rdf:resource="http://www.ontologylibrary.mil/CommonCore/Mid/QualityOntology#RadiationQuality"/>
        <rdfs:comment>A physical quality that inheres in an bearer by virtue of how that bearer interacts with electromagnetic radiation.</rdfs:comment>
    </owl:Class>
    


    <!-- http://www.ontologylibrary.mil/CommonCore/Mid/QualityOntology#Elongated -->

    <owl:Class rdf:about="http://www.ontologylibrary.mil/CommonCore/Mid/QualityOntology#Elongated">
        <rdfs:label>Elongated</rdfs:label>
        <rdfs:subClassOf rdf:resource="http://www.ontologylibrary.mil/CommonCore/Mid/QualityOntology#Shape"/>
        <rdfs:comment>A quality inhering in a bearer by virtue of the bearer&apos;s length being notably higher than its width.</rdfs:comment>
    </owl:Class>
    


    <!-- http://www.ontologylibrary.mil/CommonCore/Mid/QualityOntology#EmmisionWavelength -->

    <owl:Class rdf:about="http://www.ontologylibrary.mil/CommonCore/Mid/QualityOntology#EmmisionWavelength">
        <rdfs:label>Emmision Wavelength</rdfs:label>
        <rdfs:subClassOf rdf:resource="http://www.ontologylibrary.mil/CommonCore/Mid/QualityOntology#RadiationEmittingQuality"/>
        <rdfs:comment>The specific wavelength of light emitted by a fluorescent molecule, such as a labelled probe, upon absorption of light at the (higher) excitation wavelength.</rdfs:comment>
    </owl:Class>
    


    <!-- http://www.ontologylibrary.mil/CommonCore/Mid/QualityOntology#ExtremeUltravioletLightFrequency -->

    <owl:Class rdf:about="http://www.ontologylibrary.mil/CommonCore/Mid/QualityOntology#ExtremeUltravioletLightFrequency">
        <rdfs:label>Extreme Ultraviolet Light Frequency</rdfs:label>
        <rdfs:subClassOf rdf:resource="http://www.ontologylibrary.mil/CommonCore/Mid/QualityOntology#UltravioletLightFrequency"/>
    </owl:Class>
    


    <!-- http://www.ontologylibrary.mil/CommonCore/Mid/QualityOntology#ExtremelyHighFrequency -->

    <owl:Class rdf:about="http://www.ontologylibrary.mil/CommonCore/Mid/QualityOntology#ExtremelyHighFrequency">
        <rdfs:label>Extremely High Frequency</rdfs:label>
        <rdfs:subClassOf rdf:resource="http://www.ontologylibrary.mil/CommonCore/Mid/QualityOntology#RadioFrequency"/>
    </owl:Class>
    


    <!-- http://www.ontologylibrary.mil/CommonCore/Mid/QualityOntology#ExtremelyLowFrequency -->

    <owl:Class rdf:about="http://www.ontologylibrary.mil/CommonCore/Mid/QualityOntology#ExtremelyLowFrequency">
        <rdfs:label>Extremely Low Frequency</rdfs:label>
        <rdfs:subClassOf rdf:resource="http://www.ontologylibrary.mil/CommonCore/Mid/QualityOntology#RadioFrequency"/>
    </owl:Class>
    


    <!-- http://www.ontologylibrary.mil/CommonCore/Mid/QualityOntology#FanShaped -->

    <owl:Class rdf:about="http://www.ontologylibrary.mil/CommonCore/Mid/QualityOntology#FanShaped">
        <rdfs:label>FanShaped</rdfs:label>
        <rdfs:subClassOf rdf:resource="http://www.ontologylibrary.mil/CommonCore/Mid/QualityOntology#TwoDimensionalShape"/>
        <rdfs:comment>A quality inhering in a bearer that is shaped in the form of a fan.</rdfs:comment>
    </owl:Class>
    


    <!-- http://www.ontologylibrary.mil/CommonCore/Mid/QualityOntology#FarInfraredLightFrequency -->

    <owl:Class rdf:about="http://www.ontologylibrary.mil/CommonCore/Mid/QualityOntology#FarInfraredLightFrequency">
        <rdfs:label>Far Infrared Light Frequency</rdfs:label>
        <rdfs:subClassOf rdf:resource="http://www.ontologylibrary.mil/CommonCore/Mid/QualityOntology#InfraredLightFrequency"/>
    </owl:Class>
    


    <!-- http://www.ontologylibrary.mil/CommonCore/Mid/QualityOntology#Fatigability -->

    <owl:Class rdf:about="http://www.ontologylibrary.mil/CommonCore/Mid/QualityOntology#Fatigability">
        <rdfs:label>Fatigability</rdfs:label>
        <rdfs:subClassOf rdf:resource="http://www.ontologylibrary.mil/CommonCore/Mid/QualityOntology#Strength"/>
        <rdfs:comment>A strength quality inhering in a bearer by virtue of the bearer&apos;s tendency to lose strength.</rdfs:comment>
    </owl:Class>
    


    <!-- http://www.ontologylibrary.mil/CommonCore/Mid/QualityOntology#Flat -->

    <owl:Class rdf:about="http://www.ontologylibrary.mil/CommonCore/Mid/QualityOntology#Flat">
        <rdfs:subClassOf rdf:resource="http://www.ontologylibrary.mil/CommonCore/Mid/QualityOntology#Shape"/>
    </owl:Class>
    


    <!-- http://www.ontologylibrary.mil/CommonCore/Mid/QualityOntology#Fluorescence -->

    <owl:Class rdf:about="http://www.ontologylibrary.mil/CommonCore/Mid/QualityOntology#Fluorescence">
        <rdfs:label>Fluorescence</rdfs:label>
        <rdfs:subClassOf rdf:resource="http://www.ontologylibrary.mil/CommonCore/Mid/QualityOntology#LuminousFlux"/>
        <rdfs:comment>A luminous flux quality inhering in a bearer by virtue of the bearer&apos;s emitting longer wavelength light following the absorption of shorter wavelength radiation; fluorescence is common with aromatic compounds with several rings joined together.</rdfs:comment>
    </owl:Class>
    


    <!-- http://www.ontologylibrary.mil/CommonCore/Mid/QualityOntology#Fluorescent -->

    <owl:Class rdf:about="http://www.ontologylibrary.mil/CommonCore/Mid/QualityOntology#Fluorescent">
        <rdfs:label>Fluorescent</rdfs:label>
        <rdfs:subClassOf rdf:resource="http://www.ontologylibrary.mil/CommonCore/Mid/QualityOntology#Fluorescence"/>
        <rdfs:comment>A fluorescence quality inhering in a bearer by virtue of emitting light during exposure to radiation from an external source.</rdfs:comment>
    </owl:Class>
    


    <!-- http://www.ontologylibrary.mil/CommonCore/Mid/QualityOntology#Focus -->

    <owl:Class rdf:about="http://www.ontologylibrary.mil/CommonCore/Mid/QualityOntology#Focus">
        <rdfs:label>Focus</rdfs:label>
        <rdfs:subClassOf rdf:resource="http://www.ontologylibrary.mil/CommonCore/Mid/QualityOntology#OpticalQuality"/>
        <rdfs:comment>An optical quality where light rays originating from a point on the object converge.</rdfs:comment>
    </owl:Class>
    


    <!-- http://www.ontologylibrary.mil/CommonCore/Mid/QualityOntology#Focused -->

    <owl:Class rdf:about="http://www.ontologylibrary.mil/CommonCore/Mid/QualityOntology#Focused">
        <rdfs:label>Focused</rdfs:label>
        <rdfs:subClassOf rdf:resource="http://www.ontologylibrary.mil/CommonCore/Mid/QualityOntology#Focus"/>
        <rdfs:comment>An optical quality inhering in a bearer by virtue of the bearer&apos;s having focus.</rdfs:comment>
    </owl:Class>
    


    <!-- http://www.ontologylibrary.mil/CommonCore/Mid/QualityOntology#Folded -->

    <owl:Class rdf:about="http://www.ontologylibrary.mil/CommonCore/Mid/QualityOntology#Folded">
        <rdfs:subClassOf rdf:resource="http://www.ontologylibrary.mil/CommonCore/Mid/QualityOntology#Shape"/>
    </owl:Class>
    


    <!-- http://www.ontologylibrary.mil/CommonCore/Mid/QualityOntology#ForwardScatter -->

    <owl:Class rdf:about="http://www.ontologylibrary.mil/CommonCore/Mid/QualityOntology#ForwardScatter">
        <rdfs:label>Forward Scatter</rdfs:label>
        <rdfs:subClassOf rdf:resource="http://www.ontologylibrary.mil/CommonCore/Mid/QualityOntology#RadiationReflectiveQuality"/>
        <rdfs:comment>A reflectivity quality inhering in light by virtue of the bearer&apos;s scattering occurring at small angle to the incident beam.</rdfs:comment>
    </owl:Class>
    


    <!-- http://www.ontologylibrary.mil/CommonCore/Mid/QualityOntology#Frequency -->

    <owl:Class rdf:about="http://www.ontologylibrary.mil/CommonCore/Mid/QualityOntology#Frequency">
        <rdfs:label>Frequency</rdfs:label>
        <rdfs:subClassOf rdf:resource="&obo;BFO_0000144"/>
        <rdfs:comment>A physical quality which inheres in a bearer by virtue of the number of the bearer&apos;s repetitive actions in a particular time.</rdfs:comment>
    </owl:Class>
    


    <!-- http://www.ontologylibrary.mil/CommonCore/Mid/QualityOntology#FullSpectrumElectromagneticRadiationQuality -->

    <owl:Class rdf:about="http://www.ontologylibrary.mil/CommonCore/Mid/QualityOntology#FullSpectrumElectromagneticRadiationQuality">
        <rdfs:label>FullSpectrum Em Radiation Quality</rdfs:label>
        <rdfs:subClassOf rdf:resource="http://www.ontologylibrary.mil/CommonCore/Mid/QualityOntology#ElectromagneticRadiationQuality"/>
        <rdfs:comment>An EM radiation quality that is independent of the EM wavelength range.</rdfs:comment>
    </owl:Class>
    


    <!-- http://www.ontologylibrary.mil/CommonCore/Mid/QualityOntology#GammaRayFrequency -->

    <owl:Class rdf:about="http://www.ontologylibrary.mil/CommonCore/Mid/QualityOntology#GammaRayFrequency">
        <rdfs:label>Gamma Ray Frequency</rdfs:label>
        <rdfs:subClassOf rdf:resource="http://www.ontologylibrary.mil/CommonCore/Mid/QualityOntology#Frequency"/>
    </owl:Class>
    


    <!-- http://www.ontologylibrary.mil/CommonCore/Mid/QualityOntology#Glistening -->

    <owl:Class rdf:about="http://www.ontologylibrary.mil/CommonCore/Mid/QualityOntology#Glistening">
        <rdfs:label>Glistening</rdfs:label>
        <rdfs:subClassOf rdf:resource="http://www.ontologylibrary.mil/CommonCore/Mid/QualityOntology#Reflectivity"/>
        <rdfs:comment>A reflectivity quality inhering in a bearer by virtue of the bearer&apos;s reflecting lots of light.</rdfs:comment>
    </owl:Class>
    


    <!-- http://www.ontologylibrary.mil/CommonCore/Mid/QualityOntology#GoldColor -->

    <owl:Class rdf:about="http://www.ontologylibrary.mil/CommonCore/Mid/QualityOntology#GoldColor">
        <rdfs:label>Gold Color</rdfs:label>
        <rdfs:subClassOf rdf:resource="http://www.ontologylibrary.mil/CommonCore/Mid/QualityOntology#ColorHue"/>
    </owl:Class>
    


    <!-- http://www.ontologylibrary.mil/CommonCore/Mid/QualityOntology#Green -->

    <owl:Class rdf:about="http://www.ontologylibrary.mil/CommonCore/Mid/QualityOntology#Green">
        <rdfs:label>Green</rdfs:label>
        <rdfs:subClassOf rdf:resource="http://www.ontologylibrary.mil/CommonCore/Mid/QualityOntology#ColorHue"/>
        <rdfs:comment>A color hue with medium-low wavelength of that portion of the visible spectrum lying between yellow and blue, evoked in the human observer by radiant energy with wavelengths of approximately 490 to 570 nanometers.</rdfs:comment>
    </owl:Class>
    


    <!-- http://www.ontologylibrary.mil/CommonCore/Mid/QualityOntology#Grey -->

    <owl:Class rdf:about="http://www.ontologylibrary.mil/CommonCore/Mid/QualityOntology#Grey">
        <rdfs:label>Grey</rdfs:label>
        <rdfs:subClassOf rdf:resource="http://www.ontologylibrary.mil/CommonCore/Mid/QualityOntology#ColorHue"/>
        <rdfs:comment>A color between white and black colors.</rdfs:comment>
    </owl:Class>
    


    <!-- http://www.ontologylibrary.mil/CommonCore/Mid/QualityOntology#Hard -->

    <owl:Class rdf:about="http://www.ontologylibrary.mil/CommonCore/Mid/QualityOntology#Hard">
        <rdfs:label>Hard</rdfs:label>
        <rdfs:subClassOf rdf:resource="http://www.ontologylibrary.mil/CommonCore/Mid/QualityOntology#Hardness"/>
        <rdfs:comment>A hardness quality of being rigid and resistant to pressure.</rdfs:comment>
    </owl:Class>
    


    <!-- http://www.ontologylibrary.mil/CommonCore/Mid/QualityOntology#HardXrayFrequency -->

    <owl:Class rdf:about="http://www.ontologylibrary.mil/CommonCore/Mid/QualityOntology#HardXrayFrequency">
        <rdfs:label>Hard X-ray Frequency</rdfs:label>
        <rdfs:subClassOf rdf:resource="http://www.ontologylibrary.mil/CommonCore/Mid/QualityOntology#XrayFrequency"/>
    </owl:Class>
    


    <!-- http://www.ontologylibrary.mil/CommonCore/Mid/QualityOntology#Hardness -->

    <owl:Class rdf:about="http://www.ontologylibrary.mil/CommonCore/Mid/QualityOntology#Hardness">
        <rdfs:label>Hardness</rdfs:label>
        <rdfs:subClassOf rdf:resource="http://www.ontologylibrary.mil/CommonCore/Mid/QualityOntology#PhysicalQuality"/>
        <rdfs:comment>A physical quality inhering in a bearer by virtue of its capability of being turned, bowed, or twisted without breaking.</rdfs:comment>
    </owl:Class>
    


    <!-- http://www.ontologylibrary.mil/CommonCore/Mid/QualityOntology#Hazel -->

    <owl:Class rdf:about="http://www.ontologylibrary.mil/CommonCore/Mid/QualityOntology#Hazel">
        <rdfs:label rdf:datatype="&xsd;string">Hazel</rdfs:label>
        <rdfs:subClassOf rdf:resource="http://www.ontologylibrary.mil/CommonCore/Mid/QualityOntology#ColorHue"/>
        <rdfs:comment rdf:datatype="&xsd;string">Definition: A mixture of Brown and Green</rdfs:comment>
    </owl:Class>
    


    <!-- http://www.ontologylibrary.mil/CommonCore/Mid/QualityOntology#Height -->

    <owl:Class rdf:about="http://www.ontologylibrary.mil/CommonCore/Mid/QualityOntology#Height">
        <rdfs:label>Height</rdfs:label>
        <rdfs:subClassOf rdf:resource="http://www.ontologylibrary.mil/CommonCore/Mid/QualityOntology#OneDimensionalExtent"/>
        <rdfs:comment>A 1D extent quality inhering in a bearer by virtue of the bearer&apos;s vertical dimension of extension.</rdfs:comment>
    </owl:Class>
    


    <!-- http://www.ontologylibrary.mil/CommonCore/Mid/QualityOntology#HighBrightness -->

    <owl:Class rdf:about="http://www.ontologylibrary.mil/CommonCore/Mid/QualityOntology#HighBrightness">
        <rdfs:label>High Brightness</rdfs:label>
        <rdfs:subClassOf rdf:resource="http://www.ontologylibrary.mil/CommonCore/Mid/QualityOntology#ColorBrightness"/>
        <rdfs:comment>A color brightness which is relatively high.</rdfs:comment>
    </owl:Class>
    


    <!-- http://www.ontologylibrary.mil/CommonCore/Mid/QualityOntology#HighFrequency -->

    <owl:Class rdf:about="http://www.ontologylibrary.mil/CommonCore/Mid/QualityOntology#HighFrequency">
        <rdfs:label>High Frequency</rdfs:label>
        <rdfs:subClassOf rdf:resource="http://www.ontologylibrary.mil/CommonCore/Mid/QualityOntology#RadioFrequency"/>
    </owl:Class>
    


    <!-- http://www.ontologylibrary.mil/CommonCore/Mid/QualityOntology#HighSaturation -->

    <owl:Class rdf:about="http://www.ontologylibrary.mil/CommonCore/Mid/QualityOntology#HighSaturation">
        <rdfs:label>High Saturation</rdfs:label>
        <rdfs:subClassOf rdf:resource="http://www.ontologylibrary.mil/CommonCore/Mid/QualityOntology#ColorSaturation"/>
        <rdfs:comment>A color saturation which is of high purity.</rdfs:comment>
    </owl:Class>
    


    <!-- http://www.ontologylibrary.mil/CommonCore/Mid/QualityOntology#InfraredLightFrequency -->

    <owl:Class rdf:about="http://www.ontologylibrary.mil/CommonCore/Mid/QualityOntology#InfraredLightFrequency">
        <rdfs:label>Infrared Light Frequency</rdfs:label>
        <rdfs:subClassOf rdf:resource="http://www.ontologylibrary.mil/CommonCore/Mid/QualityOntology#LightFrequency"/>
    </owl:Class>
    


    <!-- http://www.ontologylibrary.mil/CommonCore/Mid/QualityOntology#Intrasonic -->

    <owl:Class rdf:about="http://www.ontologylibrary.mil/CommonCore/Mid/QualityOntology#Intrasonic">
        <rdfs:label>Intrasonic</rdfs:label>
        <rdfs:subClassOf rdf:resource="http://www.ontologylibrary.mil/CommonCore/Mid/QualityOntology#SoundFrequency"/>
        <rdfs:comment>A sound frequency in the range of 0-20 Hz.</rdfs:comment>
    </owl:Class>
    


    <!-- http://www.ontologylibrary.mil/CommonCore/Mid/QualityOntology#Kinked -->

    <owl:Class rdf:about="http://www.ontologylibrary.mil/CommonCore/Mid/QualityOntology#Kinked">
        <rdfs:label>Kinked</rdfs:label>
        <rdfs:subClassOf rdf:resource="http://www.ontologylibrary.mil/CommonCore/Mid/QualityOntology#Bent"/>
        <rdfs:comment>A shape quality inhering in a bearer by virtue of the bearer&apos;s having multiple angles in its length.</rdfs:comment>
    </owl:Class>
    


    <!-- http://www.ontologylibrary.mil/CommonCore/Mid/QualityOntology#LShaped -->

    <owl:Class rdf:about="http://www.ontologylibrary.mil/CommonCore/Mid/QualityOntology#LShaped">
        <rdfs:label>LShaped</rdfs:label>
        <rdfs:subClassOf rdf:resource="http://www.ontologylibrary.mil/CommonCore/Mid/QualityOntology#Angular"/>
        <rdfs:comment>An angular shape quality inhering in a bearer by virtue of the bearer&apos;s having a single angle in its length giving the bearer the form of the letter L.</rdfs:comment>
    </owl:Class>
    


    <!-- http://www.ontologylibrary.mil/CommonCore/Mid/QualityOntology#Length -->

    <owl:Class rdf:about="http://www.ontologylibrary.mil/CommonCore/Mid/QualityOntology#Length">
        <rdfs:label>Length</rdfs:label>
        <rdfs:subClassOf rdf:resource="http://www.ontologylibrary.mil/CommonCore/Mid/QualityOntology#OneDimensionalExtent"/>
        <rdfs:comment>A 1D extent quality which is equal to the distance between two points.</rdfs:comment>
    </owl:Class>
    


    <!-- http://www.ontologylibrary.mil/CommonCore/Mid/QualityOntology#LifeSpan -->

    <owl:Class rdf:about="http://www.ontologylibrary.mil/CommonCore/Mid/QualityOntology#LifeSpan">
        <rdfs:label>Life Span</rdfs:label>
        <rdfs:subClassOf rdf:resource="&obo;BFO_0000144"/>
        <rdfs:comment>A time quality inhering in a bearer by virtue of the bearer&apos;s expected maximum age.</rdfs:comment>
    </owl:Class>
    


    <!-- http://www.ontologylibrary.mil/CommonCore/Mid/QualityOntology#LightBlue -->

    <owl:Class rdf:about="http://www.ontologylibrary.mil/CommonCore/Mid/QualityOntology#LightBlue">
        <rdfs:label>Light Blue</rdfs:label>
        <rdfs:subClassOf rdf:resource="http://www.ontologylibrary.mil/CommonCore/Mid/QualityOntology#Blue"/>
        <rdfs:comment>A color consisting of blue hue and high brightness.</rdfs:comment>
    </owl:Class>
    


    <!-- http://www.ontologylibrary.mil/CommonCore/Mid/QualityOntology#LightBrown -->

    <owl:Class rdf:about="http://www.ontologylibrary.mil/CommonCore/Mid/QualityOntology#LightBrown">
        <rdfs:label>Light Brown</rdfs:label>
        <rdfs:subClassOf rdf:resource="http://www.ontologylibrary.mil/CommonCore/Mid/QualityOntology#Brown"/>
        <rdfs:comment>A color consisting of brown hue and high brightness.</rdfs:comment>
    </owl:Class>
    


    <!-- http://www.ontologylibrary.mil/CommonCore/Mid/QualityOntology#LightCyan -->

    <owl:Class rdf:about="http://www.ontologylibrary.mil/CommonCore/Mid/QualityOntology#LightCyan">
        <rdfs:label>Light Cyan</rdfs:label>
        <rdfs:subClassOf rdf:resource="http://www.ontologylibrary.mil/CommonCore/Mid/QualityOntology#Cyan"/>
        <rdfs:comment>A color consisting of cyan hue and high brightness.</rdfs:comment>
    </owl:Class>
    


    <!-- http://www.ontologylibrary.mil/CommonCore/Mid/QualityOntology#LightDeepPink -->

    <owl:Class rdf:about="http://www.ontologylibrary.mil/CommonCore/Mid/QualityOntology#LightDeepPink">
        <rdfs:label>Light Deep Pink</rdfs:label>
        <rdfs:subClassOf rdf:resource="http://www.ontologylibrary.mil/CommonCore/Mid/QualityOntology#Pink"/>
        <rdfs:comment>Pink color having high brightness and moderate saturation.</rdfs:comment>
    </owl:Class>
    


    <!-- http://www.ontologylibrary.mil/CommonCore/Mid/QualityOntology#LightFrequency -->

    <owl:Class rdf:about="http://www.ontologylibrary.mil/CommonCore/Mid/QualityOntology#LightFrequency">
        <rdfs:label>Light Frequency</rdfs:label>
        <rdfs:subClassOf rdf:resource="http://www.ontologylibrary.mil/CommonCore/Mid/QualityOntology#Frequency"/>
    </owl:Class>
    


    <!-- http://www.ontologylibrary.mil/CommonCore/Mid/QualityOntology#LightGreen -->

    <owl:Class rdf:about="http://www.ontologylibrary.mil/CommonCore/Mid/QualityOntology#LightGreen">
        <rdfs:label>Light Green</rdfs:label>
        <rdfs:subClassOf rdf:resource="http://www.ontologylibrary.mil/CommonCore/Mid/QualityOntology#Green"/>
        <rdfs:comment>A color consisting of green hue and high brightness.</rdfs:comment>
    </owl:Class>
    


    <!-- http://www.ontologylibrary.mil/CommonCore/Mid/QualityOntology#LightGrey -->

    <owl:Class rdf:about="http://www.ontologylibrary.mil/CommonCore/Mid/QualityOntology#LightGrey">
        <rdfs:label>Light Grey</rdfs:label>
        <rdfs:subClassOf rdf:resource="http://www.ontologylibrary.mil/CommonCore/Mid/QualityOntology#Grey"/>
        <rdfs:comment>A color consisting of grey color and high brightness.</rdfs:comment>
    </owl:Class>
    


    <!-- http://www.ontologylibrary.mil/CommonCore/Mid/QualityOntology#LightMagenta -->

    <owl:Class rdf:about="http://www.ontologylibrary.mil/CommonCore/Mid/QualityOntology#LightMagenta">
        <rdfs:label>Light Magenta</rdfs:label>
        <rdfs:subClassOf rdf:resource="http://www.ontologylibrary.mil/CommonCore/Mid/QualityOntology#Magenta"/>
        <rdfs:comment>A color consisting of magenta color and high brightness.</rdfs:comment>
    </owl:Class>
    


    <!-- http://www.ontologylibrary.mil/CommonCore/Mid/QualityOntology#LightOrange -->

    <owl:Class rdf:about="http://www.ontologylibrary.mil/CommonCore/Mid/QualityOntology#LightOrange">
        <rdfs:label>Light Orange</rdfs:label>
        <rdfs:subClassOf rdf:resource="http://www.ontologylibrary.mil/CommonCore/Mid/QualityOntology#Orange"/>
        <rdfs:comment>A color consisting of orange hue and high brightness.</rdfs:comment>
    </owl:Class>
    


    <!-- http://www.ontologylibrary.mil/CommonCore/Mid/QualityOntology#LightPurple -->

    <owl:Class rdf:about="http://www.ontologylibrary.mil/CommonCore/Mid/QualityOntology#LightPurple">
        <rdfs:label>Light Purple</rdfs:label>
        <rdfs:subClassOf rdf:resource="http://www.ontologylibrary.mil/CommonCore/Mid/QualityOntology#Purple"/>
        <rdfs:comment>A color consisting of purple color and high brightness.</rdfs:comment>
    </owl:Class>
    


    <!-- http://www.ontologylibrary.mil/CommonCore/Mid/QualityOntology#LightRed -->

    <owl:Class rdf:about="http://www.ontologylibrary.mil/CommonCore/Mid/QualityOntology#LightRed">
        <rdfs:label>Light Red</rdfs:label>
        <rdfs:subClassOf rdf:resource="http://www.ontologylibrary.mil/CommonCore/Mid/QualityOntology#Red"/>
        <rdfs:comment>A color consisting of red hue and high brightness.</rdfs:comment>
    </owl:Class>
    


    <!-- http://www.ontologylibrary.mil/CommonCore/Mid/QualityOntology#LightRedBrown -->

    <owl:Class rdf:about="http://www.ontologylibrary.mil/CommonCore/Mid/QualityOntology#LightRedBrown">
        <rdfs:label>Light Red Brown</rdfs:label>
        <rdfs:subClassOf rdf:resource="http://www.ontologylibrary.mil/CommonCore/Mid/QualityOntology#RedBrown"/>
        <rdfs:comment>A color consisting of red and brown hue and high brightness.</rdfs:comment>
    </owl:Class>
    


    <!-- http://www.ontologylibrary.mil/CommonCore/Mid/QualityOntology#LightViolet -->

    <owl:Class rdf:about="http://www.ontologylibrary.mil/CommonCore/Mid/QualityOntology#LightViolet">
        <rdfs:label>Light Violet</rdfs:label>
        <rdfs:subClassOf rdf:resource="http://www.ontologylibrary.mil/CommonCore/Mid/QualityOntology#Violet"/>
        <rdfs:comment>A color consisting of violet hue and high brightness.</rdfs:comment>
    </owl:Class>
    


    <!-- http://www.ontologylibrary.mil/CommonCore/Mid/QualityOntology#LightYellow -->

    <owl:Class rdf:about="http://www.ontologylibrary.mil/CommonCore/Mid/QualityOntology#LightYellow">
        <rdfs:label>Light Yellow</rdfs:label>
        <rdfs:subClassOf rdf:resource="http://www.ontologylibrary.mil/CommonCore/Mid/QualityOntology#Yellow"/>
        <rdfs:comment>A color consisting of yellow hue and high brightness.</rdfs:comment>
    </owl:Class>
    


    <!-- http://www.ontologylibrary.mil/CommonCore/Mid/QualityOntology#Lilac -->

    <owl:Class rdf:about="http://www.ontologylibrary.mil/CommonCore/Mid/QualityOntology#Lilac">
        <rdfs:label>Lilac</rdfs:label>
        <rdfs:subClassOf rdf:resource="http://www.ontologylibrary.mil/CommonCore/Mid/QualityOntology#Purple"/>
        <rdfs:comment>A purple color which has low saturation and low brightness.</rdfs:comment>
    </owl:Class>
    


    <!-- http://www.ontologylibrary.mil/CommonCore/Mid/QualityOntology#Linear -->

    <owl:Class rdf:about="http://www.ontologylibrary.mil/CommonCore/Mid/QualityOntology#Linear">
        <rdfs:label>Linear</rdfs:label>
        <rdfs:subClassOf rdf:resource="http://www.ontologylibrary.mil/CommonCore/Mid/QualityOntology#Shape"/>
        <rdfs:comment>A shape quality inhering in a bearer by virtue of the bearer&apos;s being narrow with the two opposite margins parallel.</rdfs:comment>
    </owl:Class>
    


    <!-- http://www.ontologylibrary.mil/CommonCore/Mid/QualityOntology#Loud -->

    <owl:Class rdf:about="http://www.ontologylibrary.mil/CommonCore/Mid/QualityOntology#Loud">
        <rdfs:label>Loud</rdfs:label>
        <rdfs:subClassOf rdf:resource="http://www.ontologylibrary.mil/CommonCore/Mid/QualityOntology#Loudness"/>
        <rdfs:comment>A sound amplitude which is relatively high.</rdfs:comment>
    </owl:Class>
    


    <!-- http://www.ontologylibrary.mil/CommonCore/Mid/QualityOntology#Loudness -->

    <owl:Class rdf:about="http://www.ontologylibrary.mil/CommonCore/Mid/QualityOntology#Loudness">
        <rdfs:subClassOf rdf:resource="http://www.ontologylibrary.mil/CommonCore/Mid/QualityOntology#SoundQuality"/>
    </owl:Class>
    


    <!-- http://www.ontologylibrary.mil/CommonCore/Mid/QualityOntology#LowBrightness -->

    <owl:Class rdf:about="http://www.ontologylibrary.mil/CommonCore/Mid/QualityOntology#LowBrightness">
        <rdfs:label>Low Brightness</rdfs:label>
        <rdfs:subClassOf rdf:resource="http://www.ontologylibrary.mil/CommonCore/Mid/QualityOntology#ColorBrightness"/>
        <rdfs:comment>A color brightness which is relatively low.</rdfs:comment>
    </owl:Class>
    


    <!-- http://www.ontologylibrary.mil/CommonCore/Mid/QualityOntology#LowFrequency -->

    <owl:Class rdf:about="http://www.ontologylibrary.mil/CommonCore/Mid/QualityOntology#LowFrequency">
        <rdfs:label>Low Frequency</rdfs:label>
        <rdfs:subClassOf rdf:resource="http://www.ontologylibrary.mil/CommonCore/Mid/QualityOntology#RadioFrequency"/>
    </owl:Class>
    


    <!-- http://www.ontologylibrary.mil/CommonCore/Mid/QualityOntology#LowSaturation -->

    <owl:Class rdf:about="http://www.ontologylibrary.mil/CommonCore/Mid/QualityOntology#LowSaturation">
        <rdfs:label>Low Saturation</rdfs:label>
        <rdfs:subClassOf rdf:resource="http://www.ontologylibrary.mil/CommonCore/Mid/QualityOntology#ColorSaturation"/>
        <rdfs:comment>A color saturation which is of low purity.</rdfs:comment>
    </owl:Class>
    


    <!-- http://www.ontologylibrary.mil/CommonCore/Mid/QualityOntology#Lowered -->

    <owl:Class rdf:about="http://www.ontologylibrary.mil/CommonCore/Mid/QualityOntology#Lowered">
        <rdfs:subClassOf rdf:resource="http://www.ontologylibrary.mil/CommonCore/Mid/QualityOntology#Shape"/>
    </owl:Class>
    


    <!-- http://www.ontologylibrary.mil/CommonCore/Mid/QualityOntology#Luminance -->

    <owl:Class rdf:about="http://www.ontologylibrary.mil/CommonCore/Mid/QualityOntology#Luminance">
        <rdfs:label>Luminance</rdfs:label>
        <rdfs:subClassOf rdf:resource="http://www.ontologylibrary.mil/CommonCore/Mid/QualityOntology#LuminousFlux"/>
        <rdfs:comment>A quality that exists by virtue of the luminous intensity per unit area projected in a given direction.</rdfs:comment>
    </owl:Class>
    


    <!-- http://www.ontologylibrary.mil/CommonCore/Mid/QualityOntology#LuminousFlux -->

    <owl:Class rdf:about="http://www.ontologylibrary.mil/CommonCore/Mid/QualityOntology#LuminousFlux">
        <rdfs:label>Luminous Flux</rdfs:label>
        <rdfs:subClassOf rdf:resource="http://www.ontologylibrary.mil/CommonCore/Mid/QualityOntology#OpticalQuality"/>
        <rdfs:comment>A scalar optical quality which obtains by the magnitude of the light emitted by the bearer.</rdfs:comment>
    </owl:Class>
    


    <!-- http://www.ontologylibrary.mil/CommonCore/Mid/QualityOntology#Magenta -->

    <owl:Class rdf:about="http://www.ontologylibrary.mil/CommonCore/Mid/QualityOntology#Magenta">
        <rdfs:label>Magenta</rdfs:label>
        <rdfs:subClassOf rdf:resource="http://www.ontologylibrary.mil/CommonCore/Mid/QualityOntology#ColorHue"/>
        <rdfs:comment>A color consisting of red and blue hues.</rdfs:comment>
    </owl:Class>
    


    <!-- http://www.ontologylibrary.mil/CommonCore/Mid/QualityOntology#Magnetic -->

    <owl:Class rdf:about="http://www.ontologylibrary.mil/CommonCore/Mid/QualityOntology#Magnetic">
        <rdfs:label>Magnetism</rdfs:label>
        <rdfs:subClassOf rdf:resource="&obo;BFO_0000017"/>
        <rdfs:comment>A physical quality inhering in a bearer by virtue of the bearer&apos;s ability or inablity to exert an attractive or repulsive force on other entities.</rdfs:comment>
    </owl:Class>
    


    <!-- http://www.ontologylibrary.mil/CommonCore/Mid/QualityOntology#Maroon -->

    <owl:Class rdf:about="http://www.ontologylibrary.mil/CommonCore/Mid/QualityOntology#Maroon">
        <rdfs:label>Maroon</rdfs:label>
        <rdfs:subClassOf rdf:resource="http://www.ontologylibrary.mil/CommonCore/Mid/QualityOntology#ColorHue"/>
        <rdfs:comment>A color consisting of purple and brown hue.</rdfs:comment>
    </owl:Class>
    


    <!-- http://www.ontologylibrary.mil/CommonCore/Mid/QualityOntology#Mass -->

    <owl:Class rdf:about="http://www.ontologylibrary.mil/CommonCore/Mid/QualityOntology#Mass">
        <rdfs:label>Mass</rdfs:label>
        <rdfs:subClassOf rdf:resource="http://www.ontologylibrary.mil/CommonCore/Mid/QualityOntology#PhysicalQuality"/>
        <rdfs:comment>A physical quality that inheres in a bearer by virtue of the proportion of the bearer&apos;s amount of matter.</rdfs:comment>
    </owl:Class>
    


    <!-- http://www.ontologylibrary.mil/CommonCore/Mid/QualityOntology#MediumFrequency -->

    <owl:Class rdf:about="http://www.ontologylibrary.mil/CommonCore/Mid/QualityOntology#MediumFrequency">
        <rdfs:label>Medium Frequency</rdfs:label>
        <rdfs:subClassOf rdf:resource="http://www.ontologylibrary.mil/CommonCore/Mid/QualityOntology#RadioFrequency"/>
    </owl:Class>
    


    <!-- http://www.ontologylibrary.mil/CommonCore/Mid/QualityOntology#MidInfraredLightFrequency -->

    <owl:Class rdf:about="http://www.ontologylibrary.mil/CommonCore/Mid/QualityOntology#MidInfraredLightFrequency">
        <rdfs:label>Mid Infrared Light Frequency</rdfs:label>
        <rdfs:subClassOf rdf:resource="http://www.ontologylibrary.mil/CommonCore/Mid/QualityOntology#InfraredLightFrequency"/>
    </owl:Class>
    


    <!-- http://www.ontologylibrary.mil/CommonCore/Mid/QualityOntology#MorphologicalQuality -->

    <owl:Class rdf:about="http://www.ontologylibrary.mil/CommonCore/Mid/QualityOntology#MorphologicalQuality">
        <rdfs:label rdf:datatype="&xsd;string">Morphological Quality</rdfs:label>
        <rdfs:subClassOf rdf:resource="&obo;BFO_0000019"/>
        <rdfs:comment>A quality of a single physical entity inhering in the bearer by virtue of the bearer&apos;s size or shape or structure.</rdfs:comment>
    </owl:Class>
    


    <!-- http://www.ontologylibrary.mil/CommonCore/Mid/QualityOntology#NearInfraredLightFrequency -->

    <owl:Class rdf:about="http://www.ontologylibrary.mil/CommonCore/Mid/QualityOntology#NearInfraredLightFrequency">
        <rdfs:label>Near Infrared Light Frequency</rdfs:label>
        <rdfs:subClassOf rdf:resource="http://www.ontologylibrary.mil/CommonCore/Mid/QualityOntology#InfraredLightFrequency"/>
    </owl:Class>
    


    <!-- http://www.ontologylibrary.mil/CommonCore/Mid/QualityOntology#NearUltravioletLightFrequency -->

    <owl:Class rdf:about="http://www.ontologylibrary.mil/CommonCore/Mid/QualityOntology#NearUltravioletLightFrequency">
        <rdfs:label>Near Ultraviolet Light Frequency</rdfs:label>
        <rdfs:subClassOf rdf:resource="http://www.ontologylibrary.mil/CommonCore/Mid/QualityOntology#UltravioletLightFrequency"/>
    </owl:Class>
    


    <!-- http://www.ontologylibrary.mil/CommonCore/Mid/QualityOntology#ObjectAggregateAmount -->

    <owl:Class rdf:about="http://www.ontologylibrary.mil/CommonCore/Mid/QualityOntology#ObjectAggregateAmount">
        <rdfs:label rdf:datatype="&xsd;string">Object Aggregate Amount</rdfs:label>
        <rdfs:subClassOf rdf:resource="http://www.ontologylibrary.mil/CommonCore/Mid/QualityOntology#Amount"/>
        <rdfs:comment rdf:datatype="&xsd;string">An Amount that inheres in some Object Aggregate, or in other words the number of discrete parts of an object.</rdfs:comment>
    </owl:Class>
    


    <!-- http://www.ontologylibrary.mil/CommonCore/Mid/QualityOntology#Oblong -->

    <owl:Class rdf:about="http://www.ontologylibrary.mil/CommonCore/Mid/QualityOntology#Oblong">
        <rdfs:label>Oblong</rdfs:label>
        <rdfs:subClassOf rdf:resource="http://www.ontologylibrary.mil/CommonCore/Mid/QualityOntology#TwoDimensionalShape"/>
        <rdfs:comment>A shape quality inhering in a bearer by virtue of the bearer&apos;s having a somewhat elongated form with approximately parallel sides.</rdfs:comment>
    </owl:Class>
    


    <!-- http://www.ontologylibrary.mil/CommonCore/Mid/QualityOntology#Obstructed -->

    <owl:Class rdf:about="http://www.ontologylibrary.mil/CommonCore/Mid/QualityOntology#Obstructed">
        <rdfs:label>Obstructed</rdfs:label>
        <rdfs:subClassOf rdf:resource="http://www.ontologylibrary.mil/CommonCore/Mid/QualityOntology#Closed"/>
        <rdfs:comment>A morphological quality inhering in a bearer by virtue of the bearer&apos;s being blocked or filled with obstacles or an obstacle.</rdfs:comment>
    </owl:Class>
    


    <!-- http://www.ontologylibrary.mil/CommonCore/Mid/QualityOntology#Ochre -->

    <owl:Class rdf:about="http://www.ontologylibrary.mil/CommonCore/Mid/QualityOntology#Ochre">
        <rdfs:label>Ochre</rdfs:label>
        <rdfs:subClassOf rdf:resource="http://www.ontologylibrary.mil/CommonCore/Mid/QualityOntology#YellowOrange"/>
        <rdfs:comment>A moderate yellow-orange to orange color.</rdfs:comment>
    </owl:Class>
    


    <!-- http://www.ontologylibrary.mil/CommonCore/Mid/QualityOntology#OneDimensionalExtent -->

    <owl:Class rdf:about="http://www.ontologylibrary.mil/CommonCore/Mid/QualityOntology#OneDimensionalExtent">
        <rdfs:label rdf:datatype="&xsd;string">One Dimensional Extent</rdfs:label>
        <rdfs:subClassOf rdf:resource="http://www.ontologylibrary.mil/CommonCore/Mid/QualityOntology#Size"/>
        <rdfs:comment>A size quality inhering in an bearer by virtue of the bearer&apos;s extension in one dimension.</rdfs:comment>
    </owl:Class>
    


    <!-- http://www.ontologylibrary.mil/CommonCore/Mid/QualityOntology#Opacity -->

    <owl:Class rdf:about="http://www.ontologylibrary.mil/CommonCore/Mid/QualityOntology#Opacity">
        <rdfs:label>Opacity</rdfs:label>
        <rdfs:subClassOf rdf:resource="http://www.ontologylibrary.mil/CommonCore/Mid/QualityOntology#OpticalQuality"/>
        <rdfs:comment>An optical quality which obtains by virtue of the ability of the bearer to absorb visible light.</rdfs:comment>
    </owl:Class>
    


    <!-- http://www.ontologylibrary.mil/CommonCore/Mid/QualityOntology#Opaque -->

    <owl:Class rdf:about="http://www.ontologylibrary.mil/CommonCore/Mid/QualityOntology#Opaque">
        <rdfs:label>Opaque</rdfs:label>
        <rdfs:subClassOf rdf:resource="http://www.ontologylibrary.mil/CommonCore/Mid/QualityOntology#Opacity"/>
        <rdfs:comment>A optical quality inhering in a bearer by virtue of the bearer&apos;s not being clear; not transmitting or reflecting light or radiant energy.</rdfs:comment>
    </owl:Class>
    


    <!-- http://www.ontologylibrary.mil/CommonCore/Mid/QualityOntology#Open -->

    <owl:Class rdf:about="http://www.ontologylibrary.mil/CommonCore/Mid/QualityOntology#Open">
        <rdfs:label>Open</rdfs:label>
        <rdfs:subClassOf rdf:resource="http://www.ontologylibrary.mil/CommonCore/Mid/QualityOntology#Closure"/>
        <rdfs:comment>A morphological quality inhering in a bearer by virtue of the bearer&apos;s affording unobstructed passage or view.</rdfs:comment>
    </owl:Class>
    


    <!-- http://www.ontologylibrary.mil/CommonCore/Mid/QualityOntology#OpticalQuality -->

    <owl:Class rdf:about="http://www.ontologylibrary.mil/CommonCore/Mid/QualityOntology#OpticalQuality">
        <rdfs:label>Optical Quality</rdfs:label>
        <rdfs:subClassOf rdf:resource="http://www.ontologylibrary.mil/CommonCore/Mid/QualityOntology#ElectromagneticRadiationQuality"/>
        <rdfs:comment>An EM radiation quality in which the EM radiation is within the fiat range of the spectrum visible deemed to be light.</rdfs:comment>
    </owl:Class>
    


    <!-- http://www.ontologylibrary.mil/CommonCore/Mid/QualityOntology#Orange -->

    <owl:Class rdf:about="http://www.ontologylibrary.mil/CommonCore/Mid/QualityOntology#Orange">
        <rdfs:label>Orange</rdfs:label>
        <rdfs:subClassOf rdf:resource="http://www.ontologylibrary.mil/CommonCore/Mid/QualityOntology#ColorHue"/>
        <rdfs:comment>A color hue with high-medium wavelength that of that portion of the visible spectrum lying between red and yellow, evoked in the human observer by radiant energy with wavelengths of approximately 585 to 620 nanometers.</rdfs:comment>
    </owl:Class>
    


    <!-- http://www.ontologylibrary.mil/CommonCore/Mid/QualityOntology#PalePink -->

    <owl:Class rdf:about="http://www.ontologylibrary.mil/CommonCore/Mid/QualityOntology#PalePink">
        <rdfs:label>Pale Pink</rdfs:label>
        <rdfs:subClassOf rdf:resource="http://www.ontologylibrary.mil/CommonCore/Mid/QualityOntology#Pink"/>
        <rdfs:comment>Pink color having high brightness and low saturation.</rdfs:comment>
    </owl:Class>
    


    <!-- http://www.ontologylibrary.mil/CommonCore/Mid/QualityOntology#Perimeter -->

    <owl:Class rdf:about="http://www.ontologylibrary.mil/CommonCore/Mid/QualityOntology#Perimeter">
        <rdfs:label>Perimeter</rdfs:label>
        <rdfs:subClassOf rdf:resource="http://www.ontologylibrary.mil/CommonCore/Mid/QualityOntology#Length"/>
        <rdfs:comment>An 1D extent quality inhering in twodimensional bearer by virtue of being equal to the distance around it.</rdfs:comment>
    </owl:Class>
    


    <!-- http://www.ontologylibrary.mil/CommonCore/Mid/QualityOntology#Phosphorescence -->

    <owl:Class rdf:about="http://www.ontologylibrary.mil/CommonCore/Mid/QualityOntology#Phosphorescence">
        <rdfs:label>Phosphorescence</rdfs:label>
        <rdfs:subClassOf rdf:resource="http://www.ontologylibrary.mil/CommonCore/Mid/QualityOntology#Fluorescence"/>
        <rdfs:comment>A fluorescence in which the emittence continues after the absorption has ceased.</rdfs:comment>
    </owl:Class>
    


    <!-- http://www.ontologylibrary.mil/CommonCore/Mid/QualityOntology#PhysicalQuality -->

    <owl:Class rdf:about="http://www.ontologylibrary.mil/CommonCore/Mid/QualityOntology#PhysicalQuality">
        <rdfs:label>Physical Quality</rdfs:label>
        <rdfs:subClassOf rdf:resource="&obo;BFO_0000019"/>
        <rdfs:comment>A quality of a single physical entity that exists through action of continuants at the physical level of organisation.</rdfs:comment>
    </owl:Class>
    


    <!-- http://www.ontologylibrary.mil/CommonCore/Mid/QualityOntology#Pink -->

    <owl:Class rdf:about="http://www.ontologylibrary.mil/CommonCore/Mid/QualityOntology#Pink">
        <rdfs:label>Pink</rdfs:label>
        <rdfs:subClassOf rdf:resource="http://www.ontologylibrary.mil/CommonCore/Mid/QualityOntology#Red"/>
        <rdfs:comment>Red color having medium to high brightness and low to moderate saturation.</rdfs:comment>
    </owl:Class>
    


    <!-- http://www.ontologylibrary.mil/CommonCore/Mid/QualityOntology#Pitch -->

    <owl:Class rdf:about="http://www.ontologylibrary.mil/CommonCore/Mid/QualityOntology#Pitch">
        <rdfs:subClassOf rdf:resource="http://www.ontologylibrary.mil/CommonCore/Mid/QualityOntology#SoundQuality"/>
    </owl:Class>
    


    <!-- http://www.ontologylibrary.mil/CommonCore/Mid/QualityOntology#Pointed -->

    <owl:Class rdf:about="http://www.ontologylibrary.mil/CommonCore/Mid/QualityOntology#Pointed">
        <rdfs:label>Punctiform</rdfs:label>
        <rdfs:subClassOf rdf:resource="http://www.ontologylibrary.mil/CommonCore/Mid/QualityOntology#Shape"/>
        <rdfs:comment>A shape quality inhering in a bearer by virtue of the bearer&apos;s having a pointed end</rdfs:comment>
    </owl:Class>
    


    <!-- http://www.ontologylibrary.mil/CommonCore/Mid/QualityOntology#ProcessAggregateAmount -->

    <owl:Class rdf:about="http://www.ontologylibrary.mil/CommonCore/Mid/QualityOntology#ProcessAggregateAmount">
        <rdfs:label rdf:datatype="&xsd;string">Process Aggregate Amount</rdfs:label>
        <rdfs:subClassOf rdf:resource="http://www.ontologylibrary.mil/CommonCore/Mid/QualityOntology#Amount"/>
        <rdfs:comment rdf:datatype="&xsd;string">An Amount that inheres in some Process Aggregate by virtue of number of sub-processes.</rdfs:comment>
    </owl:Class>
    


    <!-- http://www.ontologylibrary.mil/CommonCore/Mid/QualityOntology#Protruding -->

    <owl:Class rdf:about="http://www.ontologylibrary.mil/CommonCore/Mid/QualityOntology#Protruding">
        <rdfs:label>Protruding</rdfs:label>
        <rdfs:subClassOf rdf:resource="http://www.ontologylibrary.mil/CommonCore/Mid/QualityOntology#Shape"/>
        <rdfs:comment>A shape quality inhering in a bearer by virtue of the bearer&apos;s extending out above or beyond a surface or boundary it normally occupies.</rdfs:comment>
    </owl:Class>
    


    <!-- http://www.ontologylibrary.mil/CommonCore/Mid/QualityOntology#Purple -->

    <owl:Class rdf:about="http://www.ontologylibrary.mil/CommonCore/Mid/QualityOntology#Purple">
        <rdfs:label>Purple</rdfs:label>
        <rdfs:subClassOf rdf:resource="http://www.ontologylibrary.mil/CommonCore/Mid/QualityOntology#ColorHue"/>
        <rdfs:comment>A color that falls about midway between red and blue in hue.</rdfs:comment>
    </owl:Class>
    


    <!-- http://www.ontologylibrary.mil/CommonCore/Mid/QualityOntology#Quadrangular -->

    <owl:Class rdf:about="http://www.ontologylibrary.mil/CommonCore/Mid/QualityOntology#Quadrangular">
        <rdfs:label>Quadrangular</rdfs:label>
        <rdfs:subClassOf rdf:resource="http://www.ontologylibrary.mil/CommonCore/Mid/QualityOntology#TwoDimensionalShape"/>
        <rdfs:comment>A shape quality inhering in a bearer by virtue of the bearer&apos;s having four angles and four sides.</rdfs:comment>
    </owl:Class>
    


    <!-- http://www.ontologylibrary.mil/CommonCore/Mid/QualityOntology#Quiet -->

    <owl:Class rdf:about="http://www.ontologylibrary.mil/CommonCore/Mid/QualityOntology#Quiet">
        <rdfs:label>Quiet</rdfs:label>
        <rdfs:subClassOf rdf:resource="http://www.ontologylibrary.mil/CommonCore/Mid/QualityOntology#Loudness"/>
        <rdfs:comment>A sound amplitude which is relatively low.</rdfs:comment>
    </owl:Class>
    


    <!-- http://www.ontologylibrary.mil/CommonCore/Mid/QualityOntology#RadiationEmittingIntensityQuality -->

    <owl:Class rdf:about="http://www.ontologylibrary.mil/CommonCore/Mid/QualityOntology#RadiationEmittingIntensityQuality">
        <rdfs:label>Radiation Emitting Intensity Quality</rdfs:label>
        <rdfs:subClassOf rdf:resource="http://www.ontologylibrary.mil/CommonCore/Mid/QualityOntology#RadiationEmittingQuality"/>
        <rdfs:comment>A radiation emitting quality which obtains by the intensity of the bearer emitted radiation.</rdfs:comment>
    </owl:Class>
    


    <!-- http://www.ontologylibrary.mil/CommonCore/Mid/QualityOntology#RadiationEmittingQuality -->

    <owl:Class rdf:about="http://www.ontologylibrary.mil/CommonCore/Mid/QualityOntology#RadiationEmittingQuality">
        <rdfs:label>Radiation Emitting Quality</rdfs:label>
        <rdfs:subClassOf rdf:resource="http://www.ontologylibrary.mil/CommonCore/Mid/QualityOntology#FullSpectrumElectromagneticRadiationQuality"/>
        <rdfs:comment>A scalar EM radiation quality which obtains by the capacity of the bearer to emit radiation.</rdfs:comment>
    </owl:Class>
    


    <!-- http://www.ontologylibrary.mil/CommonCore/Mid/QualityOntology#RadiationQuality -->

    <owl:Class rdf:about="http://www.ontologylibrary.mil/CommonCore/Mid/QualityOntology#RadiationQuality">
        <rdfs:label>Radiation Quality</rdfs:label>
        <rdfs:subClassOf rdf:resource="&obo;BFO_0000017"/>
        <rdfs:comment>A quality that inheres in an bearer by virtue of how that bearer interacts with radiation.</rdfs:comment>
    </owl:Class>
    


    <!-- http://www.ontologylibrary.mil/CommonCore/Mid/QualityOntology#RadiationReflectiveQuality -->

    <owl:Class rdf:about="http://www.ontologylibrary.mil/CommonCore/Mid/QualityOntology#RadiationReflectiveQuality">
        <rdfs:label>Radiation Reflective Quality</rdfs:label>
        <rdfs:subClassOf rdf:resource="http://www.ontologylibrary.mil/CommonCore/Mid/QualityOntology#FullSpectrumElectromagneticRadiationQuality"/>
        <rdfs:comment>A scalar EM radiation quality which obtains by the capacity of the bearer to scatter or reflect radiation.</rdfs:comment>
    </owl:Class>
    


    <!-- http://www.ontologylibrary.mil/CommonCore/Mid/QualityOntology#RadioFrequency -->

    <owl:Class rdf:about="http://www.ontologylibrary.mil/CommonCore/Mid/QualityOntology#RadioFrequency">
        <rdfs:label>Radio Frequency</rdfs:label>
        <rdfs:subClassOf rdf:resource="http://www.ontologylibrary.mil/CommonCore/Mid/QualityOntology#Frequency"/>
    </owl:Class>
    


    <!-- http://www.ontologylibrary.mil/CommonCore/Mid/QualityOntology#Radioactive -->

    <owl:Class rdf:about="http://www.ontologylibrary.mil/CommonCore/Mid/QualityOntology#Radioactive">
        <rdfs:label>Radioactive</rdfs:label>
        <rdfs:subClassOf rdf:resource="http://www.ontologylibrary.mil/CommonCore/Mid/QualityOntology#RadiationQuality"/>
        <rdfs:comment>A radiation quality inhering in bearer by virtue of the bearer&apos;s exhibiting or being caused by radioactivity.</rdfs:comment>
    </owl:Class>
    


    <!-- http://www.ontologylibrary.mil/CommonCore/Mid/QualityOntology#Radiopacity -->

    <owl:Class rdf:about="http://www.ontologylibrary.mil/CommonCore/Mid/QualityOntology#Radiopacity">
        <rdfs:label>Radiopacity</rdfs:label>
        <rdfs:subClassOf rdf:resource="http://www.ontologylibrary.mil/CommonCore/Mid/QualityOntology#ElectromagneticRadiationQuality"/>
        <rdfs:comment>A quality inhering in a bearer by virtue of the bearer&apos;s relative inability of electromagnetism to pass through a particular material, particularly X-rays.</rdfs:comment>
    </owl:Class>
    


    <!-- http://www.ontologylibrary.mil/CommonCore/Mid/QualityOntology#Raised -->

    <owl:Class rdf:about="http://www.ontologylibrary.mil/CommonCore/Mid/QualityOntology#Raised">
        <rdfs:label>Raised</rdfs:label>
        <rdfs:subClassOf rdf:resource="http://www.ontologylibrary.mil/CommonCore/Mid/QualityOntology#Shape"/>
        <rdfs:comment>A shape quality inhering in a colony by virtue of the bearer&apos;s appearing above the medium surface with terraced edges.</rdfs:comment>
    </owl:Class>
    


    <!-- http://www.ontologylibrary.mil/CommonCore/Mid/QualityOntology#Red -->

    <owl:Class rdf:about="http://www.ontologylibrary.mil/CommonCore/Mid/QualityOntology#Red">
        <rdfs:label>Red</rdfs:label>
        <rdfs:subClassOf rdf:resource="http://www.ontologylibrary.mil/CommonCore/Mid/QualityOntology#ColorHue"/>
        <rdfs:comment>A color hue with high wavelength of the long-wave end of the visible spectrum, evoked in the human observer by radiant energy with wavelengths of approximately 630 to 750 nanometers.</rdfs:comment>
    </owl:Class>
    


    <!-- http://www.ontologylibrary.mil/CommonCore/Mid/QualityOntology#RedBrown -->

    <owl:Class rdf:about="http://www.ontologylibrary.mil/CommonCore/Mid/QualityOntology#RedBrown">
        <rdfs:label>Red Brown</rdfs:label>
        <rdfs:subClassOf rdf:resource="http://www.ontologylibrary.mil/CommonCore/Mid/QualityOntology#Brown"/>
        <rdfs:comment>A color consisting of red and brown hue.</rdfs:comment>
    </owl:Class>
    


    <!-- http://www.ontologylibrary.mil/CommonCore/Mid/QualityOntology#Reflectivity -->

    <owl:Class rdf:about="http://www.ontologylibrary.mil/CommonCore/Mid/QualityOntology#Reflectivity">
        <rdfs:label>Reflectivity</rdfs:label>
        <rdfs:subClassOf rdf:resource="http://www.ontologylibrary.mil/CommonCore/Mid/QualityOntology#RadiationReflectiveQuality"/>
        <rdfs:comment>A radiation reflective quality inhering in a bearer by virtue of the ratio of the energy of a wave reflected from its surface to the energy possessed by the wave striking the bearer&apos;s surface.</rdfs:comment>
    </owl:Class>
    


    <!-- http://www.ontologylibrary.mil/CommonCore/Mid/QualityOntology#Refractile -->

    <owl:Class rdf:about="http://www.ontologylibrary.mil/CommonCore/Mid/QualityOntology#Refractile">
        <rdfs:label>Refractile</rdfs:label>
        <rdfs:subClassOf rdf:resource="http://www.ontologylibrary.mil/CommonCore/Mid/QualityOntology#Refractivity"/>
        <rdfs:comment>A reflectivity quality inhering in the bearer by virtue of the bearer&apos;s ability to refract light.</rdfs:comment>
    </owl:Class>
    


    <!-- http://www.ontologylibrary.mil/CommonCore/Mid/QualityOntology#Refractivity -->

    <owl:Class rdf:about="http://www.ontologylibrary.mil/CommonCore/Mid/QualityOntology#Refractivity">
        <rdfs:label>Refractivity</rdfs:label>
        <rdfs:subClassOf rdf:resource="http://www.ontologylibrary.mil/CommonCore/Mid/QualityOntology#RadiationReflectiveQuality"/>
        <rdfs:comment>A physical quality that inheres in propagating wave (light or sound) virtue of the bearer&apos;s change in direction when passing from one medium to another.</rdfs:comment>
    </owl:Class>
    


    <!-- http://www.ontologylibrary.mil/CommonCore/Mid/QualityOntology#Rosy -->

    <owl:Class rdf:about="http://www.ontologylibrary.mil/CommonCore/Mid/QualityOntology#Rosy">
        <rdfs:label>Rosy</rdfs:label>
        <rdfs:subClassOf rdf:resource="http://www.ontologylibrary.mil/CommonCore/Mid/QualityOntology#ColorHue"/>
        <rdfs:comment>A color hue consisting of red hue and yellow hue and high brightness.</rdfs:comment>
    </owl:Class>
    


    <!-- http://www.ontologylibrary.mil/CommonCore/Mid/QualityOntology#Rough -->

    <owl:Class rdf:about="http://www.ontologylibrary.mil/CommonCore/Mid/QualityOntology#Rough">
        <rdfs:label>Rough</rdfs:label>
        <rdfs:subClassOf rdf:resource="http://www.ontologylibrary.mil/CommonCore/Mid/QualityOntology#Texture"/>
        <rdfs:comment>A texture quality inhering in a bearer by virtue of the bearer&apos;s irregular surface.</rdfs:comment>
    </owl:Class>
    


    <!-- http://www.ontologylibrary.mil/CommonCore/Mid/QualityOntology#Round -->

    <owl:Class rdf:about="http://www.ontologylibrary.mil/CommonCore/Mid/QualityOntology#Round">
        <rdfs:label>Round</rdfs:label>
        <rdfs:subClassOf rdf:resource="http://www.ontologylibrary.mil/CommonCore/Mid/QualityOntology#TwoDimensionalShape"/>
        <rdfs:comment>A shape quality inhering in a bearer by virtue of the bearer&apos;s being such that every part of the surface or the circumference is equidistant from the center.</rdfs:comment>
    </owl:Class>
    


    <!-- http://www.ontologylibrary.mil/CommonCore/Mid/QualityOntology#SaturatedBlue -->

    <owl:Class rdf:about="http://www.ontologylibrary.mil/CommonCore/Mid/QualityOntology#SaturatedBlue">
        <rdfs:label>Saturated Blue</rdfs:label>
        <rdfs:subClassOf rdf:resource="http://www.ontologylibrary.mil/CommonCore/Mid/QualityOntology#Blue"/>
        <rdfs:comment>A color consisting of blue hue and high saturation.</rdfs:comment>
    </owl:Class>
    


    <!-- http://www.ontologylibrary.mil/CommonCore/Mid/QualityOntology#SaturatedBrown -->

    <owl:Class rdf:about="http://www.ontologylibrary.mil/CommonCore/Mid/QualityOntology#SaturatedBrown">
        <rdfs:label>Saturated Brown</rdfs:label>
        <rdfs:subClassOf rdf:resource="http://www.ontologylibrary.mil/CommonCore/Mid/QualityOntology#Brown"/>
        <rdfs:comment>A color consisting of brown hue and high saturation.</rdfs:comment>
    </owl:Class>
    


    <!-- http://www.ontologylibrary.mil/CommonCore/Mid/QualityOntology#SaturatedCyan -->

    <owl:Class rdf:about="http://www.ontologylibrary.mil/CommonCore/Mid/QualityOntology#SaturatedCyan">
        <rdfs:label>Saturated Cyan</rdfs:label>
        <rdfs:subClassOf rdf:resource="http://www.ontologylibrary.mil/CommonCore/Mid/QualityOntology#Cyan"/>
        <rdfs:comment>A color consisting of cyan colour and high saturation.</rdfs:comment>
    </owl:Class>
    


    <!-- http://www.ontologylibrary.mil/CommonCore/Mid/QualityOntology#SaturatedGreen -->

    <owl:Class rdf:about="http://www.ontologylibrary.mil/CommonCore/Mid/QualityOntology#SaturatedGreen">
        <rdfs:label>Saturated Green</rdfs:label>
        <rdfs:subClassOf rdf:resource="http://www.ontologylibrary.mil/CommonCore/Mid/QualityOntology#Green"/>
        <rdfs:comment>A color consisting of green hue and high saturation.</rdfs:comment>
    </owl:Class>
    


    <!-- http://www.ontologylibrary.mil/CommonCore/Mid/QualityOntology#SaturatedMagenta -->

    <owl:Class rdf:about="http://www.ontologylibrary.mil/CommonCore/Mid/QualityOntology#SaturatedMagenta">
        <rdfs:label>Saturated Magenta</rdfs:label>
        <rdfs:subClassOf rdf:resource="http://www.ontologylibrary.mil/CommonCore/Mid/QualityOntology#Magenta"/>
        <rdfs:comment>A color consisting of magenta color and high saturation.</rdfs:comment>
    </owl:Class>
    


    <!-- http://www.ontologylibrary.mil/CommonCore/Mid/QualityOntology#SaturatedOrange -->

    <owl:Class rdf:about="http://www.ontologylibrary.mil/CommonCore/Mid/QualityOntology#SaturatedOrange">
        <rdfs:label>Saturated Orange</rdfs:label>
        <rdfs:subClassOf rdf:resource="http://www.ontologylibrary.mil/CommonCore/Mid/QualityOntology#Orange"/>
        <rdfs:comment>A color consisting of orange hue and high saturation.</rdfs:comment>
    </owl:Class>
    


    <!-- http://www.ontologylibrary.mil/CommonCore/Mid/QualityOntology#SaturatedPurple -->

    <owl:Class rdf:about="http://www.ontologylibrary.mil/CommonCore/Mid/QualityOntology#SaturatedPurple">
        <rdfs:label>Saturated Purple</rdfs:label>
        <rdfs:subClassOf rdf:resource="http://www.ontologylibrary.mil/CommonCore/Mid/QualityOntology#Purple"/>
        <rdfs:comment>A color consisting of purple color and high saturation.</rdfs:comment>
    </owl:Class>
    


    <!-- http://www.ontologylibrary.mil/CommonCore/Mid/QualityOntology#SaturatedRed -->

    <owl:Class rdf:about="http://www.ontologylibrary.mil/CommonCore/Mid/QualityOntology#SaturatedRed">
        <rdfs:label>Saturated Red</rdfs:label>
        <rdfs:subClassOf rdf:resource="http://www.ontologylibrary.mil/CommonCore/Mid/QualityOntology#Red"/>
        <rdfs:comment>A color consisting of red hue and high saturation.</rdfs:comment>
    </owl:Class>
    


    <!-- http://www.ontologylibrary.mil/CommonCore/Mid/QualityOntology#SaturatedViolet -->

    <owl:Class rdf:about="http://www.ontologylibrary.mil/CommonCore/Mid/QualityOntology#SaturatedViolet">
        <rdfs:label>Saturated Violet</rdfs:label>
        <rdfs:subClassOf rdf:resource="http://www.ontologylibrary.mil/CommonCore/Mid/QualityOntology#Violet"/>
        <rdfs:comment>A color consisting of violet hue and high saturation.</rdfs:comment>
    </owl:Class>
    


    <!-- http://www.ontologylibrary.mil/CommonCore/Mid/QualityOntology#SaturatedYellow -->

    <owl:Class rdf:about="http://www.ontologylibrary.mil/CommonCore/Mid/QualityOntology#SaturatedYellow">
        <rdfs:label>Saturated Yellow</rdfs:label>
        <rdfs:subClassOf rdf:resource="http://www.ontologylibrary.mil/CommonCore/Mid/QualityOntology#Yellow"/>
        <rdfs:comment>A color consisting of yellow hue and high saturation.</rdfs:comment>
    </owl:Class>
    


    <!-- http://www.ontologylibrary.mil/CommonCore/Mid/QualityOntology#Semicircular -->

    <owl:Class rdf:about="http://www.ontologylibrary.mil/CommonCore/Mid/QualityOntology#Semicircular">
        <rdfs:label>Semicircular</rdfs:label>
        <rdfs:subClassOf rdf:resource="http://www.ontologylibrary.mil/CommonCore/Mid/QualityOntology#TwoDimensionalShape"/>
        <rdfs:comment>A 2D shape quality inhering in a bearer by virtue of the bearer&apos;s having shape or form of half a circle.</rdfs:comment>
    </owl:Class>
    


    <!-- http://www.ontologylibrary.mil/CommonCore/Mid/QualityOntology#Serrated -->

    <owl:Class rdf:about="http://www.ontologylibrary.mil/CommonCore/Mid/QualityOntology#Serrated">
        <rdfs:label>Serrated</rdfs:label>
        <rdfs:subClassOf rdf:resource="http://www.ontologylibrary.mil/CommonCore/Mid/QualityOntology#Shape"/>
        <rdfs:comment>A shape quality inhering in a bearer by virtue of having sharp straightedged teeth pointing to the apex.</rdfs:comment>
    </owl:Class>
    


    <!-- http://www.ontologylibrary.mil/CommonCore/Mid/QualityOntology#Shape -->

    <owl:Class rdf:about="http://www.ontologylibrary.mil/CommonCore/Mid/QualityOntology#Shape">
        <rdfs:label>Shape</rdfs:label>
        <rdfs:subClassOf rdf:resource="http://www.ontologylibrary.mil/CommonCore/Mid/QualityOntology#MorphologicalQuality"/>
        <rdfs:comment>A morphological quality inhering in a bearer by virtue of the bearer&apos;s ratios of distances between its features (points edges surfaces and also holes etc).</rdfs:comment>
    </owl:Class>
    


    <!-- http://www.ontologylibrary.mil/CommonCore/Mid/QualityOntology#Sharp -->

    <owl:Class rdf:about="http://www.ontologylibrary.mil/CommonCore/Mid/QualityOntology#Sharp">
        <rdfs:label>Sharp</rdfs:label>
        <rdfs:subClassOf rdf:resource="http://www.ontologylibrary.mil/CommonCore/Mid/QualityOntology#Sharpness"/>
        <rdfs:comment>A shape quality inhering in a bearer by virtue of the bearer&apos;s terminating in a point or edge.</rdfs:comment>
    </owl:Class>
    


    <!-- http://www.ontologylibrary.mil/CommonCore/Mid/QualityOntology#Sharpness -->

    <owl:Class rdf:about="http://www.ontologylibrary.mil/CommonCore/Mid/QualityOntology#Sharpness">
        <rdfs:label>Sharpness</rdfs:label>
        <rdfs:subClassOf rdf:resource="http://www.ontologylibrary.mil/CommonCore/Mid/QualityOntology#Shape"/>
        <rdfs:comment>A shape quality inhering in a bearer by virtue of the bearer&apos;s having a sharp or tapered end or point.</rdfs:comment>
    </owl:Class>
    


    <!-- http://www.ontologylibrary.mil/CommonCore/Mid/QualityOntology#SideScatter -->

    <owl:Class rdf:about="http://www.ontologylibrary.mil/CommonCore/Mid/QualityOntology#SideScatter">
        <rdfs:label>Side Scatter</rdfs:label>
        <rdfs:subClassOf rdf:resource="http://www.ontologylibrary.mil/CommonCore/Mid/QualityOntology#RadiationReflectiveQuality"/>
        <rdfs:comment>A reflective quality that is the light scattering occurring at wide angle (around 90 degrees) to the incident beam.</rdfs:comment>
    </owl:Class>
    


    <!-- http://www.ontologylibrary.mil/CommonCore/Mid/QualityOntology#SilverColor -->

    <owl:Class rdf:about="http://www.ontologylibrary.mil/CommonCore/Mid/QualityOntology#SilverColor">
        <rdfs:label>Silver Color</rdfs:label>
        <rdfs:subClassOf rdf:resource="http://www.ontologylibrary.mil/CommonCore/Mid/QualityOntology#ColorHue"/>
    </owl:Class>
    


    <!-- http://www.ontologylibrary.mil/CommonCore/Mid/QualityOntology#Size -->

    <owl:Class rdf:about="http://www.ontologylibrary.mil/CommonCore/Mid/QualityOntology#Size">
        <rdfs:label>Size</rdfs:label>
        <rdfs:subClassOf rdf:resource="http://www.ontologylibrary.mil/CommonCore/Mid/QualityOntology#MorphologicalQuality"/>
        <rdfs:comment>A morphology quality inhering in a bearer by virtue of the bearer&apos;s physical magnitude.</rdfs:comment>
    </owl:Class>
    


    <!-- http://www.ontologylibrary.mil/CommonCore/Mid/QualityOntology#Slender -->

    <owl:Class rdf:about="http://www.ontologylibrary.mil/CommonCore/Mid/QualityOntology#Slender">
        <rdfs:label>Slender</rdfs:label>
        <rdfs:subClassOf rdf:resource="http://www.ontologylibrary.mil/CommonCore/Mid/QualityOntology#Shape"/>
        <rdfs:comment>A shape quality inhering in a bearer by virtue of the bearer&apos;s being &quot;small or narrow in circumference or width in proportion to length or height.</rdfs:comment>
    </owl:Class>
    


    <!-- http://www.ontologylibrary.mil/CommonCore/Mid/QualityOntology#Sloped -->

    <owl:Class rdf:about="http://www.ontologylibrary.mil/CommonCore/Mid/QualityOntology#Sloped">
        <rdfs:label>Sloped</rdfs:label>
        <rdfs:subClassOf rdf:resource="http://www.ontologylibrary.mil/CommonCore/Mid/QualityOntology#Shape"/>
        <rdfs:comment>A shape quality inhering in a bearer by virtue of the bearer&apos;s having an oblique or slanted direction.</rdfs:comment>
    </owl:Class>
    


    <!-- http://www.ontologylibrary.mil/CommonCore/Mid/QualityOntology#Smooth -->

    <owl:Class rdf:about="http://www.ontologylibrary.mil/CommonCore/Mid/QualityOntology#Smooth">
        <rdfs:label>Smooth</rdfs:label>
        <rdfs:subClassOf rdf:resource="http://www.ontologylibrary.mil/CommonCore/Mid/QualityOntology#Texture"/>
        <rdfs:comment>A texture quality inhering in a bearer by virtue of the bearer&apos;s processing a surface free of roughness or irregularities.</rdfs:comment>
    </owl:Class>
    


    <!-- http://www.ontologylibrary.mil/CommonCore/Mid/QualityOntology#Soft -->

    <owl:Class rdf:about="http://www.ontologylibrary.mil/CommonCore/Mid/QualityOntology#Soft">
        <rdfs:label>Soft</rdfs:label>
        <rdfs:subClassOf rdf:resource="http://www.ontologylibrary.mil/CommonCore/Mid/QualityOntology#Hardness"/>
        <rdfs:comment>A hardness quality of giving little resistance to pressure.</rdfs:comment>
    </owl:Class>
    


    <!-- http://www.ontologylibrary.mil/CommonCore/Mid/QualityOntology#SoftXrayFrequency -->

    <owl:Class rdf:about="http://www.ontologylibrary.mil/CommonCore/Mid/QualityOntology#SoftXrayFrequency">
        <rdfs:label>Soft X-ray Frequency</rdfs:label>
        <rdfs:subClassOf rdf:resource="http://www.ontologylibrary.mil/CommonCore/Mid/QualityOntology#XrayFrequency"/>
    </owl:Class>
    


    <!-- http://www.ontologylibrary.mil/CommonCore/Mid/QualityOntology#Sonic -->

    <owl:Class rdf:about="http://www.ontologylibrary.mil/CommonCore/Mid/QualityOntology#Sonic">
        <rdfs:label>Sonic</rdfs:label>
        <rdfs:subClassOf rdf:resource="http://www.ontologylibrary.mil/CommonCore/Mid/QualityOntology#SoundFrequency"/>
        <rdfs:comment>A sound frequency in the range of 20 - 20 000 Hz.</rdfs:comment>
    </owl:Class>
    


    <!-- http://www.ontologylibrary.mil/CommonCore/Mid/QualityOntology#SoundFrequency -->

    <owl:Class rdf:about="http://www.ontologylibrary.mil/CommonCore/Mid/QualityOntology#SoundFrequency">
        <rdfs:label>Sound Frequency</rdfs:label>
        <rdfs:subClassOf rdf:resource="http://www.ontologylibrary.mil/CommonCore/Mid/QualityOntology#Frequency"/>
        <rdfs:comment>The frequency of transmitted vibrations.</rdfs:comment>
    </owl:Class>
    


    <!-- http://www.ontologylibrary.mil/CommonCore/Mid/QualityOntology#SoundQuality -->

    <owl:Class rdf:about="http://www.ontologylibrary.mil/CommonCore/Mid/QualityOntology#SoundQuality">
        <rdfs:label>Sound Quality</rdfs:label>
        <rdfs:subClassOf rdf:resource="&obo;BFO_0000144"/>
        <rdfs:comment>A quality inhering in a bearer by virtue of vibration, as perceived by the sense of hearing.</rdfs:comment>
    </owl:Class>
    


    <!-- http://www.ontologylibrary.mil/CommonCore/Mid/QualityOntology#SoundWavelength -->

    <owl:Class rdf:about="http://www.ontologylibrary.mil/CommonCore/Mid/QualityOntology#SoundWavelength">
        <rdfs:label>Sound Wavelength</rdfs:label>
        <rdfs:subClassOf rdf:resource="http://www.ontologylibrary.mil/CommonCore/Mid/QualityOntology#SoundQuality"/>
        <rdfs:comment>A physical quality which is equal to the quotient of the speed of a sound wave divided by its wavelength.</rdfs:comment>
    </owl:Class>
    


    <!-- http://www.ontologylibrary.mil/CommonCore/Mid/QualityOntology#Spherical -->

    <owl:Class rdf:about="http://www.ontologylibrary.mil/CommonCore/Mid/QualityOntology#Spherical">
        <rdfs:subClassOf rdf:resource="http://www.ontologylibrary.mil/CommonCore/Mid/QualityOntology#ThreeDimensionalShape"/>
    </owl:Class>
    


    <!-- http://www.ontologylibrary.mil/CommonCore/Mid/QualityOntology#Split -->

    <owl:Class rdf:about="http://www.ontologylibrary.mil/CommonCore/Mid/QualityOntology#Split">
        <rdfs:label>Split</rdfs:label>
        <rdfs:subClassOf rdf:resource="http://www.ontologylibrary.mil/CommonCore/Mid/QualityOntology#Shape"/>
        <rdfs:comment>A shape quality inhering in a bearer by virtue of the bearer&apos;s being divided or broken up into parts or divisions.</rdfs:comment>
    </owl:Class>
    


    <!-- http://www.ontologylibrary.mil/CommonCore/Mid/QualityOntology#StarShaped -->

    <owl:Class rdf:about="http://www.ontologylibrary.mil/CommonCore/Mid/QualityOntology#StarShaped">
        <rdfs:label>Star Shaped</rdfs:label>
        <rdfs:subClassOf rdf:resource="http://www.ontologylibrary.mil/CommonCore/Mid/QualityOntology#Shape"/>
        <rdfs:comment>A shape quality inhering in a bearer by virtue of the bearer&apos;s being arranged like rays or radii; radiating from a common center.</rdfs:comment>
    </owl:Class>
    


    <!-- http://www.ontologylibrary.mil/CommonCore/Mid/QualityOntology#Straight -->

    <owl:Class rdf:about="http://www.ontologylibrary.mil/CommonCore/Mid/QualityOntology#Straight">
        <rdfs:label>Straight</rdfs:label>
        <rdfs:subClassOf rdf:resource="http://www.ontologylibrary.mil/CommonCore/Mid/QualityOntology#Shape"/>
        <rdfs:comment>A shape quality inhering in a bearer by virtue of the bearer&apos;s being free of curves bends or angles.</rdfs:comment>
    </owl:Class>
    


    <!-- http://www.ontologylibrary.mil/CommonCore/Mid/QualityOntology#Strength -->

    <owl:Class rdf:about="http://www.ontologylibrary.mil/CommonCore/Mid/QualityOntology#Strength">
        <rdfs:label>Strength</rdfs:label>
        <rdfs:subClassOf rdf:resource="&obo;BFO_0000017"/>
        <rdfs:comment>A quality inhering in a bearer by virtue of the bearer&apos;s power or force.</rdfs:comment>
    </owl:Class>
    


    <!-- http://www.ontologylibrary.mil/CommonCore/Mid/QualityOntology#SuperHighFrequency -->

    <owl:Class rdf:about="http://www.ontologylibrary.mil/CommonCore/Mid/QualityOntology#SuperHighFrequency">
        <rdfs:label>Super High  Frequency</rdfs:label>
        <rdfs:subClassOf rdf:resource="http://www.ontologylibrary.mil/CommonCore/Mid/QualityOntology#RadioFrequency"/>
    </owl:Class>
    


    <!-- http://www.ontologylibrary.mil/CommonCore/Mid/QualityOntology#SuperLowFrequency -->

    <owl:Class rdf:about="http://www.ontologylibrary.mil/CommonCore/Mid/QualityOntology#SuperLowFrequency">
        <rdfs:label>Super Low Frequency</rdfs:label>
        <rdfs:subClassOf rdf:resource="http://www.ontologylibrary.mil/CommonCore/Mid/QualityOntology#RadioFrequency"/>
    </owl:Class>
    


    <!-- http://www.ontologylibrary.mil/CommonCore/Mid/QualityOntology#SurfaceTension -->

    <owl:Class rdf:about="http://www.ontologylibrary.mil/CommonCore/Mid/QualityOntology#SurfaceTension">
        <rdfs:label>Surface Tension</rdfs:label>
        <rdfs:subClassOf rdf:resource="http://www.ontologylibrary.mil/CommonCore/Mid/QualityOntology#PhysicalQuality"/>
        <rdfs:comment>A physical quality inhering in a liquid by virtue of the bearer&apos;s ability to attraction of molecules at its surface as a result of unbalanced molecular cohesive forces.</rdfs:comment>
    </owl:Class>
    


    <!-- http://www.ontologylibrary.mil/CommonCore/Mid/QualityOntology#Temperature -->

    <owl:Class rdf:about="http://www.ontologylibrary.mil/CommonCore/Mid/QualityOntology#Temperature">
        <rdfs:label>Temperature</rdfs:label>
        <rdfs:subClassOf rdf:resource="http://www.ontologylibrary.mil/CommonCore/Mid/QualityOntology#PhysicalQuality"/>
        <rdfs:comment>A physical quality of the thermal energy of a system.</rdfs:comment>
    </owl:Class>
    


    <!-- http://www.ontologylibrary.mil/CommonCore/Mid/QualityOntology#Texture -->

    <owl:Class rdf:about="http://www.ontologylibrary.mil/CommonCore/Mid/QualityOntology#Texture">
        <rdfs:label>Texture</rdfs:label>
        <rdfs:subClassOf rdf:resource="http://www.ontologylibrary.mil/CommonCore/Mid/QualityOntology#MorphologicalQuality"/>
        <rdfs:comment>A morphologic quality inhering in a bearer by virtue of the bearer&apos;s relative size organization and distribution of its surface elements or the representation or invention of the appearance of its surface; visual and tactile surface characteristics.</rdfs:comment>
    </owl:Class>
    


    <!-- http://www.ontologylibrary.mil/CommonCore/Mid/QualityOntology#Thickness -->

    <owl:Class rdf:about="http://www.ontologylibrary.mil/CommonCore/Mid/QualityOntology#Thickness">
        <rdfs:label>Thickness</rdfs:label>
        <rdfs:subClassOf rdf:resource="http://www.ontologylibrary.mil/CommonCore/Mid/QualityOntology#OneDimensionalExtent"/>
        <rdfs:comment>A 1D extent quality which is equal to the dimension through an object as opposed to its length or width.</rdfs:comment>
    </owl:Class>
    


    <!-- http://www.ontologylibrary.mil/CommonCore/Mid/QualityOntology#ThreeDimensionalExtent -->

    <owl:Class rdf:about="http://www.ontologylibrary.mil/CommonCore/Mid/QualityOntology#ThreeDimensionalExtent">
        <rdfs:label rdf:datatype="&xsd;string">Three Dimensional Extent</rdfs:label>
        <rdfs:subClassOf rdf:resource="http://www.ontologylibrary.mil/CommonCore/Mid/QualityOntology#Size"/>
        <obo:IAO_0000118>Volume</obo:IAO_0000118>
        <rdfs:comment>A size quality inhering in an bearer by virtue of the bearer&apos;s extension in three dimensions.</rdfs:comment>
    </owl:Class>
    


    <!-- http://www.ontologylibrary.mil/CommonCore/Mid/QualityOntology#ThreeDimensionalShape -->

    <owl:Class rdf:about="http://www.ontologylibrary.mil/CommonCore/Mid/QualityOntology#ThreeDimensionalShape">
        <rdfs:subClassOf rdf:resource="http://www.ontologylibrary.mil/CommonCore/Mid/QualityOntology#Shape"/>
    </owl:Class>
    


    <!-- http://www.ontologylibrary.mil/CommonCore/Mid/QualityOntology#Timbre -->

    <owl:Class rdf:about="http://www.ontologylibrary.mil/CommonCore/Mid/QualityOntology#Timbre">
        <rdfs:subClassOf rdf:resource="http://www.ontologylibrary.mil/CommonCore/Mid/QualityOntology#SoundQuality"/>
    </owl:Class>
    


    <!-- http://www.ontologylibrary.mil/CommonCore/Mid/QualityOntology#Translucent -->

    <owl:Class rdf:about="http://www.ontologylibrary.mil/CommonCore/Mid/QualityOntology#Translucent">
        <rdfs:label>Translucent</rdfs:label>
        <rdfs:subClassOf rdf:resource="http://www.ontologylibrary.mil/CommonCore/Mid/QualityOntology#Opacity"/>
        <rdfs:comment>A optical quality inhering in a bearer by virtue of the bearer&apos;s exhibiting low opacity.</rdfs:comment>
    </owl:Class>
    


    <!-- http://www.ontologylibrary.mil/CommonCore/Mid/QualityOntology#Transparent -->

    <owl:Class rdf:about="http://www.ontologylibrary.mil/CommonCore/Mid/QualityOntology#Transparent">
        <rdfs:label>Transparent</rdfs:label>
        <rdfs:subClassOf rdf:resource="http://www.ontologylibrary.mil/CommonCore/Mid/QualityOntology#Opacity"/>
        <rdfs:comment>A optical quality inhering in a bearer by virtue of the bearer&apos;s lacking opacity.</rdfs:comment>
    </owl:Class>
    


    <!-- http://www.ontologylibrary.mil/CommonCore/Mid/QualityOntology#TremendouslyHighFrequency -->

    <owl:Class rdf:about="http://www.ontologylibrary.mil/CommonCore/Mid/QualityOntology#TremendouslyHighFrequency">
        <rdfs:label>Tremendously High Frequency</rdfs:label>
        <rdfs:subClassOf rdf:resource="http://www.ontologylibrary.mil/CommonCore/Mid/QualityOntology#RadioFrequency"/>
    </owl:Class>
    


    <!-- http://www.ontologylibrary.mil/CommonCore/Mid/QualityOntology#Triangular -->

    <owl:Class rdf:about="http://www.ontologylibrary.mil/CommonCore/Mid/QualityOntology#Triangular">
        <rdfs:label>Triangular</rdfs:label>
        <rdfs:subClassOf rdf:resource="http://www.ontologylibrary.mil/CommonCore/Mid/QualityOntology#TwoDimensionalShape"/>
        <rdfs:comment>A shape quality inhering in a bearer by virtue of the bearer&apos;s having three angles.</rdfs:comment>
    </owl:Class>
    


    <!-- http://www.ontologylibrary.mil/CommonCore/Mid/QualityOntology#Truncated -->

    <owl:Class rdf:about="http://www.ontologylibrary.mil/CommonCore/Mid/QualityOntology#Truncated">
        <rdfs:label>Truncated</rdfs:label>
        <rdfs:subClassOf rdf:resource="http://www.ontologylibrary.mil/CommonCore/Mid/QualityOntology#Shape"/>
        <rdfs:comment>A shape quality inhering in a bearer by virtue of the bearer&apos;s terminating abruptly by having or as if having an end or point cut off.</rdfs:comment>
    </owl:Class>
    


    <!-- http://www.ontologylibrary.mil/CommonCore/Mid/QualityOntology#TwoDimensionalExtent -->

    <owl:Class rdf:about="http://www.ontologylibrary.mil/CommonCore/Mid/QualityOntology#TwoDimensionalExtent">
        <rdfs:label rdf:datatype="&xsd;string">Two Dimensional Extent</rdfs:label>
        <rdfs:subClassOf rdf:resource="http://www.ontologylibrary.mil/CommonCore/Mid/QualityOntology#Size"/>
        <obo:IAO_0000118>Area</obo:IAO_0000118>
        <rdfs:comment>A size quality inhering in an bearer by virtue of the bearer&apos;s extension in two dimensions.</rdfs:comment>
    </owl:Class>
    


    <!-- http://www.ontologylibrary.mil/CommonCore/Mid/QualityOntology#TwoDimensionalShape -->

    <owl:Class rdf:about="http://www.ontologylibrary.mil/CommonCore/Mid/QualityOntology#TwoDimensionalShape">
        <rdfs:label rdf:datatype="&xsd;string">Two Dimensional Shape</rdfs:label>
        <rdfs:subClassOf rdf:resource="http://www.ontologylibrary.mil/CommonCore/Mid/QualityOntology#Shape"/>
        <rdfs:comment>A shape that inheres in a 2 dimensional entity such as a cross section or projection of a 3 dimensional entity.</rdfs:comment>
    </owl:Class>
    


    <!-- http://www.ontologylibrary.mil/CommonCore/Mid/QualityOntology#UltraHighFrequency -->

    <owl:Class rdf:about="http://www.ontologylibrary.mil/CommonCore/Mid/QualityOntology#UltraHighFrequency">
        <rdfs:label>Ultra High Frequency</rdfs:label>
        <rdfs:subClassOf rdf:resource="http://www.ontologylibrary.mil/CommonCore/Mid/QualityOntology#RadioFrequency"/>
    </owl:Class>
    


    <!-- http://www.ontologylibrary.mil/CommonCore/Mid/QualityOntology#UltraLowFrequency -->

    <owl:Class rdf:about="http://www.ontologylibrary.mil/CommonCore/Mid/QualityOntology#UltraLowFrequency">
        <rdfs:label>Ultra Low Frequency</rdfs:label>
        <rdfs:subClassOf rdf:resource="http://www.ontologylibrary.mil/CommonCore/Mid/QualityOntology#RadioFrequency"/>
    </owl:Class>
    


    <!-- http://www.ontologylibrary.mil/CommonCore/Mid/QualityOntology#Ultrasonic -->

    <owl:Class rdf:about="http://www.ontologylibrary.mil/CommonCore/Mid/QualityOntology#Ultrasonic">
        <rdfs:label>Ultrasonic</rdfs:label>
        <rdfs:subClassOf rdf:resource="http://www.ontologylibrary.mil/CommonCore/Mid/QualityOntology#SoundFrequency"/>
        <rdfs:comment>A sound frequency in the range of 20 000 + Hz.</rdfs:comment>
    </owl:Class>
    


    <!-- http://www.ontologylibrary.mil/CommonCore/Mid/QualityOntology#UltravioletLightFrequency -->

    <owl:Class rdf:about="http://www.ontologylibrary.mil/CommonCore/Mid/QualityOntology#UltravioletLightFrequency">
        <rdfs:label>Ultraviolet Light Frequency</rdfs:label>
        <rdfs:subClassOf rdf:resource="http://www.ontologylibrary.mil/CommonCore/Mid/QualityOntology#LightFrequency"/>
    </owl:Class>
    


    <!-- http://www.ontologylibrary.mil/CommonCore/Mid/QualityOntology#Unbranched -->

    <owl:Class rdf:about="http://www.ontologylibrary.mil/CommonCore/Mid/QualityOntology#Unbranched">
        <rdfs:label>Unbranched</rdfs:label>
        <rdfs:subClassOf rdf:resource="http://www.ontologylibrary.mil/CommonCore/Mid/QualityOntology#Branchiness"/>
        <rdfs:comment>A branchiness quality inhering in a bearer by virtue of the bearer&apos;s lacking branches.</rdfs:comment>
    </owl:Class>
    


    <!-- http://www.ontologylibrary.mil/CommonCore/Mid/QualityOntology#Uncoiled -->

    <owl:Class rdf:about="http://www.ontologylibrary.mil/CommonCore/Mid/QualityOntology#Uncoiled">
        <rdfs:label>Uncoiled</rdfs:label>
        <rdfs:subClassOf rdf:resource="http://www.ontologylibrary.mil/CommonCore/Mid/QualityOntology#Coiling"/>
        <rdfs:comment>A shape quality inhering in a bearer by virtue of the bearer&apos;s being not curled or wound (especially in concentric rings or spirals).</rdfs:comment>
    </owl:Class>
    


    <!-- http://www.ontologylibrary.mil/CommonCore/Mid/QualityOntology#VShaped -->

    <owl:Class rdf:about="http://www.ontologylibrary.mil/CommonCore/Mid/QualityOntology#VShaped">
        <rdfs:label>VShaped</rdfs:label>
        <rdfs:subClassOf rdf:resource="http://www.ontologylibrary.mil/CommonCore/Mid/QualityOntology#Angular"/>
        <rdfs:comment>An angular shape quality inhering in a bearer by virtue of the bearer&apos;s having a single angle in its length giving the bearer the form of the letter V.</rdfs:comment>
    </owl:Class>
    


    <!-- http://www.ontologylibrary.mil/CommonCore/Mid/QualityOntology#Vermilion -->

    <owl:Class rdf:about="http://www.ontologylibrary.mil/CommonCore/Mid/QualityOntology#Vermilion">
        <rdfs:label>Vermilion</rdfs:label>
        <rdfs:subClassOf rdf:resource="http://www.ontologylibrary.mil/CommonCore/Mid/QualityOntology#ColorHue"/>
        <rdfs:comment>A color consisting of red and orange hue with a slight amount of gray.</rdfs:comment>
    </owl:Class>
    


    <!-- http://www.ontologylibrary.mil/CommonCore/Mid/QualityOntology#VeryHighFrequency -->

    <owl:Class rdf:about="http://www.ontologylibrary.mil/CommonCore/Mid/QualityOntology#VeryHighFrequency">
        <rdfs:label>Very High Frequency</rdfs:label>
        <rdfs:subClassOf rdf:resource="http://www.ontologylibrary.mil/CommonCore/Mid/QualityOntology#RadioFrequency"/>
    </owl:Class>
    


    <!-- http://www.ontologylibrary.mil/CommonCore/Mid/QualityOntology#VeryLowFrequency -->

    <owl:Class rdf:about="http://www.ontologylibrary.mil/CommonCore/Mid/QualityOntology#VeryLowFrequency">
        <rdfs:label>Very Low Frequency</rdfs:label>
        <rdfs:subClassOf rdf:resource="http://www.ontologylibrary.mil/CommonCore/Mid/QualityOntology#RadioFrequency"/>
    </owl:Class>
    


    <!-- http://www.ontologylibrary.mil/CommonCore/Mid/QualityOntology#Violet -->

    <owl:Class rdf:about="http://www.ontologylibrary.mil/CommonCore/Mid/QualityOntology#Violet">
        <rdfs:label>Violet</rdfs:label>
        <rdfs:subClassOf rdf:resource="http://www.ontologylibrary.mil/CommonCore/Mid/QualityOntology#ColorHue"/>
        <rdfs:comment>A color hue with very low wavelength of that portion of the visible spectrum lying between reddish blue or bluish purple, evoked in the human observer by radiant energy with wavelengths of approximately 420 to 380 nanometers.</rdfs:comment>
    </owl:Class>
    


    <!-- http://www.ontologylibrary.mil/CommonCore/Mid/QualityOntology#VisibleLightFrequency -->

    <owl:Class rdf:about="http://www.ontologylibrary.mil/CommonCore/Mid/QualityOntology#VisibleLightFrequency">
        <rdfs:subClassOf rdf:resource="http://www.ontologylibrary.mil/CommonCore/Mid/QualityOntology#LightFrequency"/>
    </owl:Class>
    


    <!-- http://www.ontologylibrary.mil/CommonCore/Mid/QualityOntology#Weight -->

    <owl:Class rdf:about="http://www.ontologylibrary.mil/CommonCore/Mid/QualityOntology#Weight">
        <rdfs:label>Weight</rdfs:label>
        <rdfs:subClassOf rdf:resource="http://www.ontologylibrary.mil/CommonCore/Mid/QualityOntology#PhysicalQuality"/>
        <rdfs:comment>A physical quality inhering in a bearer that has mass near a gravitational body.</rdfs:comment>
    </owl:Class>
    


    <!-- http://www.ontologylibrary.mil/CommonCore/Mid/QualityOntology#Wet -->

    <owl:Class rdf:about="http://www.ontologylibrary.mil/CommonCore/Mid/QualityOntology#Wet">
        <rdfs:label>Wet</rdfs:label>
        <rdfs:subClassOf rdf:resource="http://www.ontologylibrary.mil/CommonCore/Mid/QualityOntology#Wetness"/>
        <rdfs:comment>A wetness quality inhering in a bearer by virtue of the bearer&apos;s being covered by a liquid.</rdfs:comment>
    </owl:Class>
    


    <!-- http://www.ontologylibrary.mil/CommonCore/Mid/QualityOntology#Wetness -->

    <owl:Class rdf:about="http://www.ontologylibrary.mil/CommonCore/Mid/QualityOntology#Wetness">
        <rdfs:label>Wetness</rdfs:label>
        <rdfs:subClassOf rdf:resource="http://www.ontologylibrary.mil/CommonCore/Mid/QualityOntology#PhysicalQuality"/>
        <rdfs:comment>A quality inhering in a bearer by virtue of whether the bearer&apos;s being covered by a liquid.</rdfs:comment>
    </owl:Class>
    


    <!-- http://www.ontologylibrary.mil/CommonCore/Mid/QualityOntology#WheelShaped -->

    <owl:Class rdf:about="http://www.ontologylibrary.mil/CommonCore/Mid/QualityOntology#WheelShaped">
        <rdfs:subClassOf rdf:resource="http://www.ontologylibrary.mil/CommonCore/Mid/QualityOntology#ThreeDimensionalShape"/>
    </owl:Class>
    


    <!-- http://www.ontologylibrary.mil/CommonCore/Mid/QualityOntology#White -->

    <owl:Class rdf:about="http://www.ontologylibrary.mil/CommonCore/Mid/QualityOntology#White">
        <rdfs:label>White</rdfs:label>
        <rdfs:subClassOf rdf:resource="http://www.ontologylibrary.mil/CommonCore/Mid/QualityOntology#ColorHue"/>
        <rdfs:comment>An achromatic color of maximum brightness; the color of objects that reflect nearly all light of all visible wavelengths.</rdfs:comment>
    </owl:Class>
    


    <!-- http://www.ontologylibrary.mil/CommonCore/Mid/QualityOntology#Width -->

    <owl:Class rdf:about="http://www.ontologylibrary.mil/CommonCore/Mid/QualityOntology#Width">
        <rdfs:label>Width</rdfs:label>
        <rdfs:subClassOf rdf:resource="http://www.ontologylibrary.mil/CommonCore/Mid/QualityOntology#OneDimensionalExtent"/>
        <rdfs:comment>A 1D extent quality which is equal to the distance from one side of an object to another side which is opposite.</rdfs:comment>
    </owl:Class>
    


    <!-- http://www.ontologylibrary.mil/CommonCore/Mid/QualityOntology#WingShaped -->

    <owl:Class rdf:about="http://www.ontologylibrary.mil/CommonCore/Mid/QualityOntology#WingShaped">
        <rdfs:label>Aliform</rdfs:label>
        <rdfs:subClassOf rdf:resource="http://www.ontologylibrary.mil/CommonCore/Mid/QualityOntology#TwoDimensionalShape"/>
        <rdfs:comment>shape quality inhering in a bearer by virtue of the bearer&apos;s being shaped like a wing.</rdfs:comment>
    </owl:Class>
    


    <!-- http://www.ontologylibrary.mil/CommonCore/Mid/QualityOntology#XrayFrequency -->

    <owl:Class rdf:about="http://www.ontologylibrary.mil/CommonCore/Mid/QualityOntology#XrayFrequency">
        <rdfs:label>X-ray Frequency</rdfs:label>
        <rdfs:subClassOf rdf:resource="http://www.ontologylibrary.mil/CommonCore/Mid/QualityOntology#Frequency"/>
    </owl:Class>
    


    <!-- http://www.ontologylibrary.mil/CommonCore/Mid/QualityOntology#Yellow -->

    <owl:Class rdf:about="http://www.ontologylibrary.mil/CommonCore/Mid/QualityOntology#Yellow">
        <rdfs:label>Yellow</rdfs:label>
        <rdfs:subClassOf rdf:resource="http://www.ontologylibrary.mil/CommonCore/Mid/QualityOntology#ColorHue"/>
        <rdfs:comment>A color hue with medium wavelength of that portion of the visible spectrum lying between orange and green, evoked in the human observer by radiant energy with wavelengths of approximately 570 to 590 nanometers.</rdfs:comment>
    </owl:Class>
    


    <!-- http://www.ontologylibrary.mil/CommonCore/Mid/QualityOntology#YellowGreen -->

    <owl:Class rdf:about="http://www.ontologylibrary.mil/CommonCore/Mid/QualityOntology#YellowGreen">
        <rdfs:label>Yellow Green</rdfs:label>
        <rdfs:subClassOf rdf:resource="http://www.ontologylibrary.mil/CommonCore/Mid/QualityOntology#Green"/>
        <rdfs:comment>A color consisting of yellow and green hues.</rdfs:comment>
    </owl:Class>
    


    <!-- http://www.ontologylibrary.mil/CommonCore/Mid/QualityOntology#YellowOrange -->

    <owl:Class rdf:about="http://www.ontologylibrary.mil/CommonCore/Mid/QualityOntology#YellowOrange">
        <rdfs:label>Yellow Orange</rdfs:label>
        <rdfs:subClassOf rdf:resource="http://www.ontologylibrary.mil/CommonCore/Mid/QualityOntology#Orange"/>
        <rdfs:comment>A color consisting of yellow and orange hue.</rdfs:comment>
    </owl:Class>
</rdf:RDF>



<!-- Generated by the OWL API (version 3.5.0) http://owlapi.sourceforge.net -->

